<?xml version="1.0"?>
<rdf:RDF xmlns="http://www.semanticweb.org/ontologies/2022/2/CDS_V0.6.owl#"
     xml:base="http://www.semanticweb.org/ontologies/2022/2/CDS_V0.6.owl"
     xmlns:dc="http://purl.org/dc/elements/1.1/"
     xmlns:owl="http://www.w3.org/2002/07/owl#"
     xmlns:rdf="http://www.w3.org/1999/02/22-rdf-syntax-ns#"
     xmlns:xml="http://www.w3.org/XML/1998/namespace"
     xmlns:xsd="http://www.w3.org/2001/XMLSchema#"
     xmlns:rdfs="http://www.w3.org/2000/01/rdf-schema#">
    <owl:Ontology rdf:about="http://www.semanticweb.org/ontologies/2022/2/CDS_V0.6.owl"/>
    


    <!-- 
    ///////////////////////////////////////////////////////////////////////////////////////
    //
    // Annotation properties
    //
    ///////////////////////////////////////////////////////////////////////////////////////
     -->


    


    <!-- http://purl.org/dc/elements/1.1/contributor -->


    <owl:AnnotationProperty rdf:about="http://purl.org/dc/elements/1.1/contributor"/>
    


    <!-- 
    ///////////////////////////////////////////////////////////////////////////////////////
    //
    // Object Properties
    //
    ///////////////////////////////////////////////////////////////////////////////////////
     -->


    


    <!-- http://www.semanticweb.org/ontologies/2022/2/CDS_V0.6.owl#action_refinement -->


    <owl:ObjectProperty rdf:about="http://www.semanticweb.org/ontologies/2022/2/CDS_V0.6.owl#action_refinement">
        <rdfs:domain rdf:resource="http://www.semanticweb.org/ontologies/2022/2/CDS_V0.6.owl#Action"/>
        <rdfs:range rdf:resource="http://www.semanticweb.org/ontologies/2022/2/CDS_V0.6.owl#Abstract_Constraint"/>
        <rdfs:comment xml:lang="en">Constraint used to refine the semantics of an Action.</rdfs:comment>
    </owl:ObjectProperty>
    


    <!-- http://www.semanticweb.org/ontologies/2022/2/CDS_V0.6.owl#application -->


    <owl:ObjectProperty rdf:about="http://www.semanticweb.org/ontologies/2022/2/CDS_V0.6.owl#application">
        <rdfs:domain rdf:resource="http://www.semanticweb.org/ontologies/2022/2/CDS_V0.6.owl#Data_Service"/>
        <rdfs:range rdf:resource="http://www.semanticweb.org/ontologies/2022/2/CDS_V0.6.owl#Data_App"/>
        <rdfs:comment xml:lang="en">Function implemented by the Data Service by means of a Data App</rdfs:comment>
    </owl:ObjectProperty>
    


    <!-- http://www.semanticweb.org/ontologies/2022/2/CDS_V0.6.owl#assigneeOf -->


    <owl:ObjectProperty rdf:about="http://www.semanticweb.org/ontologies/2022/2/CDS_V0.6.owl#assigneeOf">
        <rdfs:domain rdf:resource="http://www.semanticweb.org/ontologies/2022/2/CDS_V0.6.owl#Participant"/>
        <rdfs:range rdf:resource="http://www.semanticweb.org/ontologies/2022/2/CDS_V0.6.owl#Contract"/>
        <rdfs:comment xml:lang="en">Identifies the Contract for which the identified Particpant undertakes the assignee functional role.</rdfs:comment>
    </owl:ObjectProperty>
    


    <!-- http://www.semanticweb.org/ontologies/2022/2/CDS_V0.6.owl#assignerOf -->


    <owl:ObjectProperty rdf:about="http://www.semanticweb.org/ontologies/2022/2/CDS_V0.6.owl#assignerOf">
        <rdfs:domain rdf:resource="http://www.semanticweb.org/ontologies/2022/2/CDS_V0.6.owl#Participant"/>
        <rdfs:range rdf:resource="http://www.semanticweb.org/ontologies/2022/2/CDS_V0.6.owl#Contract"/>
        <rdfs:comment xml:lang="en">Identifies the Contract for which the identified Participant undertakes the assigner functional role.</rdfs:comment>
    </owl:ObjectProperty>
    


    <!-- http://www.semanticweb.org/ontologies/2022/2/CDS_V0.6.owl#connector_reference -->


    <owl:ObjectProperty rdf:about="http://www.semanticweb.org/ontologies/2022/2/CDS_V0.6.owl#connector_reference">
        <rdfs:domain rdf:resource="http://www.semanticweb.org/ontologies/2022/2/CDS_V0.6.owl#Broker"/>
        <rdfs:range rdf:resource="http://www.semanticweb.org/ontologies/2022/2/CDS_V0.6.owl#Connector"/>
        <rdfs:comment xml:lang="en">Reference to Connectors, which are listed in the Broker.</rdfs:comment>
    </owl:ObjectProperty>
    


    <!-- http://www.semanticweb.org/ontologies/2022/2/CDS_V0.6.owl#consequence -->


    <owl:ObjectProperty rdf:about="http://www.semanticweb.org/ontologies/2022/2/CDS_V0.6.owl#consequence">
        <rdfs:domain rdf:resource="http://www.semanticweb.org/ontologies/2022/2/CDS_V0.6.owl#Duty"/>
        <rdfs:range rdf:resource="http://www.semanticweb.org/ontologies/2022/2/CDS_V0.6.owl#Duty"/>
        <rdfs:comment xml:lang="en">Relates a Duty to another Duty, the latter being a consequence of not fulfilling the former.</rdfs:comment>
    </owl:ObjectProperty>
    


    <!-- http://www.semanticweb.org/ontologies/2022/2/CDS_V0.6.owl#consumer -->


    <owl:ObjectProperty rdf:about="http://www.semanticweb.org/ontologies/2022/2/CDS_V0.6.owl#consumer">
        <rdfs:domain rdf:resource="http://www.semanticweb.org/ontologies/2022/2/CDS_V0.6.owl#Contract"/>
        <rdfs:range rdf:resource="http://www.semanticweb.org/ontologies/2022/2/CDS_V0.6.owl#Participant"/>
        <rdfs:comment xml:lang="en">Consumer of a Resource or Service that is the subject matter of the Contract. This party may differ from the Assignee specified by the Contract rules.</rdfs:comment>
    </owl:ObjectProperty>
    


    <!-- http://www.semanticweb.org/ontologies/2022/2/CDS_V0.6.owl#contract_offer -->


    <owl:ObjectProperty rdf:about="http://www.semanticweb.org/ontologies/2022/2/CDS_V0.6.owl#contract_offer">
        <rdfs:domain rdf:resource="http://www.semanticweb.org/ontologies/2022/2/CDS_V0.6.owl#Resource"/>
        <rdfs:range rdf:resource="http://www.semanticweb.org/ontologies/2022/2/CDS_V0.6.owl#Contract_offer"/>
        <rdfs:comment xml:lang="en">Reference to a Contract Offer defining the authorized use of the Resource</rdfs:comment>
    </owl:ObjectProperty>
    


    <!-- http://www.semanticweb.org/ontologies/2022/2/CDS_V0.6.owl#creator -->


    <owl:ObjectProperty rdf:about="http://www.semanticweb.org/ontologies/2022/2/CDS_V0.6.owl#creator">
        <rdfs:domain rdf:resource="http://www.semanticweb.org/ontologies/2022/2/CDS_V0.6.owl#Resource"/>
        <rdfs:range rdf:resource="http://www.semanticweb.org/ontologies/2022/2/CDS_V0.6.owl#Participant"/>
        <rdfs:comment xml:lang="en">The entity responsible for producing the resource.</rdfs:comment>
    </owl:ObjectProperty>
    


    <!-- http://www.semanticweb.org/ontologies/2022/2/CDS_V0.6.owl#curator -->


    <owl:ObjectProperty rdf:about="http://www.semanticweb.org/ontologies/2022/2/CDS_V0.6.owl#curator">
        <rdfs:domain rdf:resource="http://www.semanticweb.org/ontologies/2022/2/CDS_V0.6.owl#Ecosystem_Component"/>
        <rdfs:range rdf:resource="http://www.semanticweb.org/ontologies/2022/2/CDS_V0.6.owl#Participant"/>
        <rdfs:comment xml:lang="en">Participant responsible for the correctness of the content offered by the Ecosystem Component.</rdfs:comment>
    </owl:ObjectProperty>
    


    <!-- http://www.semanticweb.org/ontologies/2022/2/CDS_V0.6.owl#deployed -->


    <owl:ObjectProperty rdf:about="http://www.semanticweb.org/ontologies/2022/2/CDS_V0.6.owl#deployed">
        <rdfs:domain rdf:resource="http://www.semanticweb.org/ontologies/2022/2/CDS_V0.6.owl#Data_App"/>
        <rdfs:range rdf:resource="http://www.semanticweb.org/ontologies/2022/2/CDS_V0.6.owl#Connector"/>
        <rdfs:comment xml:lang="en">Data App deployed inside a Connector</rdfs:comment>
    </owl:ObjectProperty>
    


    <!-- http://www.semanticweb.org/ontologies/2022/2/CDS_V0.6.owl#exposes -->


    <owl:ObjectProperty rdf:about="http://www.semanticweb.org/ontologies/2022/2/CDS_V0.6.owl#exposes">
        <rdfs:domain rdf:resource="http://www.semanticweb.org/ontologies/2022/2/CDS_V0.6.owl#Data_Service"/>
        <rdfs:range rdf:resource="http://www.semanticweb.org/ontologies/2022/2/CDS_V0.6.owl#DataApp_Endpoint"/>
        <rdfs:comment xml:lang="en">Data App Endpoints are exposed by a Data Service to reach the relevant Data Apps.</rdfs:comment>
    </owl:ObjectProperty>
    


    <!-- http://www.semanticweb.org/ontologies/2022/2/CDS_V0.6.owl#has_action -->


    <owl:ObjectProperty rdf:about="http://www.semanticweb.org/ontologies/2022/2/CDS_V0.6.owl#has_action">
        <rdfs:domain rdf:resource="http://www.semanticweb.org/ontologies/2022/2/CDS_V0.6.owl#Rule"/>
        <rdfs:range rdf:resource="http://www.semanticweb.org/ontologies/2022/2/CDS_V0.6.owl#Action"/>
        <rdfs:comment xml:lang="en">The operation relating to the Asset for which the Rule is being subjected.</rdfs:comment>
    </owl:ObjectProperty>
    


    <!-- http://www.semanticweb.org/ontologies/2022/2/CDS_V0.6.owl#has_assignee -->


    <owl:ObjectProperty rdf:about="http://www.semanticweb.org/ontologies/2022/2/CDS_V0.6.owl#has_assignee">
        <rdfs:domain rdf:resource="http://www.semanticweb.org/ontologies/2022/2/CDS_V0.6.owl#Rule"/>
        <rdfs:range rdf:resource="http://www.semanticweb.org/ontologies/2022/2/CDS_V0.6.owl#Participant"/>
        <rdfs:comment xml:lang="en">indicates the Party that is the recipient the of Rule. For example, the Party being granted a Permission or required to fulfil an agreed Duty.</rdfs:comment>
    </owl:ObjectProperty>
    


    <!-- http://www.semanticweb.org/ontologies/2022/2/CDS_V0.6.owl#has_assigner -->


    <owl:ObjectProperty rdf:about="http://www.semanticweb.org/ontologies/2022/2/CDS_V0.6.owl#has_assigner">
        <rdfs:domain rdf:resource="http://www.semanticweb.org/ontologies/2022/2/CDS_V0.6.owl#Rule"/>
        <rdfs:range rdf:resource="http://www.semanticweb.org/ontologies/2022/2/CDS_V0.6.owl#Participant"/>
        <rdfs:comment xml:lang="en">indicates the Party that is issuing the Rule. For example, the Party granting a Permission or requiring an agreed Duty to be fulfilled.</rdfs:comment>
    </owl:ObjectProperty>
    


    <!-- http://www.semanticweb.org/ontologies/2022/2/CDS_V0.6.owl#has_connector_default_endpoint -->


    <owl:ObjectProperty rdf:about="http://www.semanticweb.org/ontologies/2022/2/CDS_V0.6.owl#has_connector_default_endpoint">
        <rdfs:domain rdf:resource="http://www.semanticweb.org/ontologies/2022/2/CDS_V0.6.owl#Connector"/>
        <rdfs:range rdf:resource="http://www.semanticweb.org/ontologies/2022/2/CDS_V0.6.owl#Connector_Endpoint"/>
        <rdfs:comment xml:lang="en">Indicates the default endpoint that should be used for basic infrastructure interactions, e.g., providing the self description.</rdfs:comment>
    </owl:ObjectProperty>
    


    <!-- http://www.semanticweb.org/ontologies/2022/2/CDS_V0.6.owl#has_constraint -->


    <owl:ObjectProperty rdf:about="http://www.semanticweb.org/ontologies/2022/2/CDS_V0.6.owl#has_constraint">
        <rdfs:domain rdf:resource="http://www.semanticweb.org/ontologies/2022/2/CDS_V0.6.owl#Rule"/>
        <rdfs:range rdf:resource="http://www.semanticweb.org/ontologies/2022/2/CDS_V0.6.owl#Abstract_Constraint"/>
        <rdfs:comment xml:lang="en">Constraints applied to a Rule</rdfs:comment>
    </owl:ObjectProperty>
    


    <!-- http://www.semanticweb.org/ontologies/2022/2/CDS_V0.6.owl#has_dataapp_default_endpoint -->


    <owl:ObjectProperty rdf:about="http://www.semanticweb.org/ontologies/2022/2/CDS_V0.6.owl#has_dataapp_default_endpoint">
        <rdfs:domain rdf:resource="http://www.semanticweb.org/ontologies/2022/2/CDS_V0.6.owl#Data_App"/>
        <rdfs:range rdf:resource="http://www.semanticweb.org/ontologies/2022/2/CDS_V0.6.owl#DataApp_Endpoint"/>
        <rdfs:comment xml:lang="en">Indicates the default endpoint that should be used for basic infrastructure interactions, e.g., providing the self description.</rdfs:comment>
    </owl:ObjectProperty>
    


    <!-- http://www.semanticweb.org/ontologies/2022/2/CDS_V0.6.owl#has_duty -->


    <owl:ObjectProperty rdf:about="http://www.semanticweb.org/ontologies/2022/2/CDS_V0.6.owl#has_duty">
        <rdfs:domain rdf:resource="http://www.semanticweb.org/ontologies/2022/2/CDS_V0.6.owl#Permission"/>
        <rdfs:range rdf:resource="http://www.semanticweb.org/ontologies/2022/2/CDS_V0.6.owl#Duty"/>
        <rdfs:comment xml:lang="en">Relates an individual Duty to a Permission.
Note: A Duty is a pre-condition which must be fulfilled in order to receive the Permission.</rdfs:comment>
    </owl:ObjectProperty>
    


    <!-- http://www.semanticweb.org/ontologies/2022/2/CDS_V0.6.owl#has_participant_certification -->


    <owl:ObjectProperty rdf:about="http://www.semanticweb.org/ontologies/2022/2/CDS_V0.6.owl#has_participant_certification">
        <rdfs:domain rdf:resource="http://www.semanticweb.org/ontologies/2022/2/CDS_V0.6.owl#Participant"/>
        <rdfs:range rdf:resource="http://www.semanticweb.org/ontologies/2022/2/CDS_V0.6.owl#Participant_Certification"/>
        <rdfs:comment xml:lang="en">Certification issued for the given Participant.</rdfs:comment>
    </owl:ObjectProperty>
    


    <!-- http://www.semanticweb.org/ontologies/2022/2/CDS_V0.6.owl#has_resource_endpoint -->


    <owl:ObjectProperty rdf:about="http://www.semanticweb.org/ontologies/2022/2/CDS_V0.6.owl#has_resource_endpoint">
        <rdfs:domain rdf:resource="http://www.semanticweb.org/ontologies/2022/2/CDS_V0.6.owl#Connector_Endpoint"/>
        <rdfs:range rdf:resource="http://www.semanticweb.org/ontologies/2022/2/CDS_V0.6.owl#Resource"/>
        <rdfs:comment xml:lang="en">Reference to the Endpoints serving the resource&apos;s content</rdfs:comment>
    </owl:ObjectProperty>
    


    <!-- http://www.semanticweb.org/ontologies/2022/2/CDS_V0.6.owl#has_target -->


    <owl:ObjectProperty rdf:about="http://www.semanticweb.org/ontologies/2022/2/CDS_V0.6.owl#has_target">
        <rdfs:domain rdf:resource="http://www.semanticweb.org/ontologies/2022/2/CDS_V0.6.owl#Rule"/>
        <rdfs:range rdf:resource="http://www.semanticweb.org/ontologies/2022/2/CDS_V0.6.owl#Resource"/>
        <rdfs:comment xml:lang="en">The subject of the policy statement. It indicates that the Resource is the primary subject to which the Rule action directly applies.
Example: the assigner Participant offers to &lt;action&gt; the target Resource</rdfs:comment>
    </owl:ObjectProperty>
    


    <!-- http://www.semanticweb.org/ontologies/2022/2/CDS_V0.6.owl#has_user -->


    <owl:ObjectProperty rdf:about="http://www.semanticweb.org/ontologies/2022/2/CDS_V0.6.owl#has_user">
        <rdfs:domain rdf:resource="http://www.semanticweb.org/ontologies/2022/2/CDS_V0.6.owl#Resource"/>
        <rdfs:range rdf:resource="http://www.semanticweb.org/ontologies/2022/2/CDS_V0.6.owl#Participant"/>
        <rdfs:comment xml:lang="en">The participant intending to use the dataThe participant intending to use the data</rdfs:comment>
    </owl:ObjectProperty>
    


    <!-- http://www.semanticweb.org/ontologies/2022/2/CDS_V0.6.owl#implies -->


    <owl:ObjectProperty rdf:about="http://www.semanticweb.org/ontologies/2022/2/CDS_V0.6.owl#implies">
        <rdfs:domain rdf:resource="http://www.semanticweb.org/ontologies/2022/2/CDS_V0.6.owl#Action"/>
        <rdfs:range rdf:resource="http://www.semanticweb.org/ontologies/2022/2/CDS_V0.6.owl#Action"/>
        <rdfs:comment xml:lang="en">Constraint used to refine the semantics of an Action.</rdfs:comment>
    </owl:ObjectProperty>
    


    <!-- http://www.semanticweb.org/ontologies/2022/2/CDS_V0.6.owl#includedIn -->


    <owl:ObjectProperty rdf:about="http://www.semanticweb.org/ontologies/2022/2/CDS_V0.6.owl#includedIn">
        <rdfs:domain rdf:resource="http://www.semanticweb.org/ontologies/2022/2/CDS_V0.6.owl#Action"/>
        <rdfs:range rdf:resource="http://www.semanticweb.org/ontologies/2022/2/CDS_V0.6.owl#Action"/>
        <rdfs:comment xml:lang="en">An Action asserts that another Action is not prohibited to enable its operational semantics.</rdfs:comment>
    </owl:ObjectProperty>
    


    <!-- http://www.semanticweb.org/ontologies/2022/2/CDS_V0.6.owl#index -->


    <owl:ObjectProperty rdf:about="http://www.semanticweb.org/ontologies/2022/2/CDS_V0.6.owl#index">
        <rdfs:domain rdf:resource="http://www.semanticweb.org/ontologies/2022/2/CDS_V0.6.owl#Broker"/>
        <rdfs:range rdf:resource="http://www.semanticweb.org/ontologies/2022/2/CDS_V0.6.owl#Data_Asset"/>
        <rdfs:comment xml:lang="en">Metadata indexing from data sources</rdfs:comment>
    </owl:ObjectProperty>
    


    <!-- http://www.semanticweb.org/ontologies/2022/2/CDS_V0.6.owl#maintainer -->


    <owl:ObjectProperty rdf:about="http://www.semanticweb.org/ontologies/2022/2/CDS_V0.6.owl#maintainer">
        <rdfs:domain rdf:resource="http://www.semanticweb.org/ontologies/2022/2/CDS_V0.6.owl#Ecosystem_Component"/>
        <rdfs:range rdf:resource="http://www.semanticweb.org/ontologies/2022/2/CDS_V0.6.owl#Participant"/>
        <rdfs:comment xml:lang="en">Participant responsible for technical maintenance of the Ecosystem Component.</rdfs:comment>
    </owl:ObjectProperty>
    


    <!-- http://www.semanticweb.org/ontologies/2022/2/CDS_V0.6.owl#memberPerson -->


    <owl:ObjectProperty rdf:about="http://www.semanticweb.org/ontologies/2022/2/CDS_V0.6.owl#memberPerson">
        <rdfs:domain rdf:resource="http://www.semanticweb.org/ontologies/2022/2/CDS_V0.6.owl#Participant"/>
        <rdfs:range rdf:resource="http://www.semanticweb.org/ontologies/2022/2/CDS_V0.6.owl#Person"/>
        <rdfs:comment xml:lang="en">A person member of Participant</rdfs:comment>
    </owl:ObjectProperty>
    


    <!-- http://www.semanticweb.org/ontologies/2022/2/CDS_V0.6.owl#obligation -->


    <owl:ObjectProperty rdf:about="http://www.semanticweb.org/ontologies/2022/2/CDS_V0.6.owl#obligation">
        <rdfs:domain rdf:resource="http://www.semanticweb.org/ontologies/2022/2/CDS_V0.6.owl#Contract"/>
        <rdfs:range rdf:resource="http://www.semanticweb.org/ontologies/2022/2/CDS_V0.6.owl#Duty"/>
        <rdfs:comment xml:lang="en">Relates an individual Duty to a Contract</rdfs:comment>
    </owl:ObjectProperty>
    


    <!-- http://www.semanticweb.org/ontologies/2022/2/CDS_V0.6.owl#operation_type -->


    <owl:ObjectProperty rdf:about="http://www.semanticweb.org/ontologies/2022/2/CDS_V0.6.owl#operation_type">
        <rdfs:domain rdf:resource="http://www.semanticweb.org/ontologies/2022/2/CDS_V0.6.owl#Data_Service"/>
        <rdfs:range rdf:resource="http://www.semanticweb.org/ontologies/2022/2/CDS_V0.6.owl#Data_Asset"/>
        <rdfs:comment xml:lang="en">Processing, distribution, and operations of a Data Asset performed by a Data Service</rdfs:comment>
    </owl:ObjectProperty>
    


    <!-- http://www.semanticweb.org/ontologies/2022/2/CDS_V0.6.owl#participant_link -->


    <owl:ObjectProperty rdf:about="http://www.semanticweb.org/ontologies/2022/2/CDS_V0.6.owl#participant_link">
        <rdfs:domain rdf:resource="http://www.semanticweb.org/ontologies/2022/2/CDS_V0.6.owl#Service_Catalogue"/>
        <rdfs:range rdf:resource="http://www.semanticweb.org/ontologies/2022/2/CDS_V0.6.owl#Participant"/>
        <rdfs:comment xml:lang="en">A Participant that is listed in the Catalogue</rdfs:comment>
    </owl:ObjectProperty>
    


    <!-- http://www.semanticweb.org/ontologies/2022/2/CDS_V0.6.owl#participant_refinement -->


    <owl:ObjectProperty rdf:about="http://www.semanticweb.org/ontologies/2022/2/CDS_V0.6.owl#participant_refinement">
        <rdfs:domain rdf:resource="http://www.semanticweb.org/ontologies/2022/2/CDS_V0.6.owl#Participant"/>
        <rdfs:range rdf:resource="http://www.semanticweb.org/ontologies/2022/2/CDS_V0.6.owl#Abstract_Constraint"/>
        <rdfs:comment xml:lang="en">Conditions which needs to be satisfied that a single Participant can be seen as a member of the subject Participant. For instance, all Participants with their headquarter in Europe might be a potential consumer of GDPR-releated data.</rdfs:comment>
    </owl:ObjectProperty>
    


    <!-- http://www.semanticweb.org/ontologies/2022/2/CDS_V0.6.owl#permission -->


    <owl:ObjectProperty rdf:about="http://www.semanticweb.org/ontologies/2022/2/CDS_V0.6.owl#permission">
        <rdfs:domain rdf:resource="http://www.semanticweb.org/ontologies/2022/2/CDS_V0.6.owl#Contract"/>
        <rdfs:range rdf:resource="http://www.semanticweb.org/ontologies/2022/2/CDS_V0.6.owl#Permission"/>
        <rdfs:comment xml:lang="en">Relates an individual Permission to a Contract</rdfs:comment>
    </owl:ObjectProperty>
    


    <!-- http://www.semanticweb.org/ontologies/2022/2/CDS_V0.6.owl#prohibition -->


    <owl:ObjectProperty rdf:about="http://www.semanticweb.org/ontologies/2022/2/CDS_V0.6.owl#prohibition">
        <rdfs:domain rdf:resource="http://www.semanticweb.org/ontologies/2022/2/CDS_V0.6.owl#Contract"/>
        <rdfs:range rdf:resource="http://www.semanticweb.org/ontologies/2022/2/CDS_V0.6.owl#Prohibition"/>
        <rdfs:comment xml:lang="en">Relates an individual Prohibition to a Contract.</rdfs:comment>
    </owl:ObjectProperty>
    


    <!-- http://www.semanticweb.org/ontologies/2022/2/CDS_V0.6.owl#provider -->


    <owl:ObjectProperty rdf:about="http://www.semanticweb.org/ontologies/2022/2/CDS_V0.6.owl#provider">
        <rdfs:domain rdf:resource="http://www.semanticweb.org/ontologies/2022/2/CDS_V0.6.owl#Contract"/>
        <rdfs:range rdf:resource="http://www.semanticweb.org/ontologies/2022/2/CDS_V0.6.owl#Participant"/>
        <rdfs:comment xml:lang="en">Provider of a Resource or Service that is the subject matter of the contract. This party may differ from the Assigner specified by the Contract rules.</rdfs:comment>
    </owl:ObjectProperty>
    


    <!-- http://www.semanticweb.org/ontologies/2022/2/CDS_V0.6.owl#publisher -->


    <owl:ObjectProperty rdf:about="http://www.semanticweb.org/ontologies/2022/2/CDS_V0.6.owl#publisher">
        <rdfs:domain rdf:resource="http://www.semanticweb.org/ontologies/2022/2/CDS_V0.6.owl#Resource"/>
        <rdfs:range rdf:resource="http://www.semanticweb.org/ontologies/2022/2/CDS_V0.6.owl#Participant"/>
        <rdfs:comment xml:lang="en">The entity responsible for making the resource available (which may differ from the sovereign).</rdfs:comment>
    </owl:ObjectProperty>
    


    <!-- http://www.semanticweb.org/ontologies/2022/2/CDS_V0.6.owl#reads -->


    <owl:ObjectProperty rdf:about="http://www.semanticweb.org/ontologies/2022/2/CDS_V0.6.owl#reads">
        <rdfs:domain rdf:resource="http://www.semanticweb.org/ontologies/2022/2/CDS_V0.6.owl#Clearing_House"/>
        <rdfs:range rdf:resource="http://www.semanticweb.org/ontologies/2022/2/CDS_V0.6.owl#Data_Service"/>
        <rdfs:comment xml:lang="en">Data Service producing a transaction (involving action, service, participant, price) from which Clearing House reads transaction information.</rdfs:comment>
    </owl:ObjectProperty>
    


    <!-- http://www.semanticweb.org/ontologies/2022/2/CDS_V0.6.owl#records -->


    <owl:ObjectProperty rdf:about="http://www.semanticweb.org/ontologies/2022/2/CDS_V0.6.owl#records">
        <rdfs:domain rdf:resource="http://www.semanticweb.org/ontologies/2022/2/CDS_V0.6.owl#Wallet"/>
        <rdfs:range rdf:resource="http://www.semanticweb.org/ontologies/2022/2/CDS_V0.6.owl#Transaction_Data"/>
        <rdfs:comment xml:lang="en">the Wallet Service records the transaction, calculating the cost consumed by the Participant on the basis of the action and its pricing strategy</rdfs:comment>
    </owl:ObjectProperty>
    


    <!-- http://www.semanticweb.org/ontologies/2022/2/CDS_V0.6.owl#refinement -->


    <owl:ObjectProperty rdf:about="http://www.semanticweb.org/ontologies/2022/2/CDS_V0.6.owl#refinement">
        <rdfs:domain rdf:resource="http://www.semanticweb.org/ontologies/2022/2/CDS_V0.6.owl#Resource"/>
        <rdfs:range rdf:resource="http://www.semanticweb.org/ontologies/2022/2/CDS_V0.6.owl#Abstract_Constraint"/>
        <rdfs:comment xml:lang="en">Constraint used to refine the semantics of Resource.</rdfs:comment>
    </owl:ObjectProperty>
    


    <!-- http://www.semanticweb.org/ontologies/2022/2/CDS_V0.6.owl#remedy -->


    <owl:ObjectProperty rdf:about="http://www.semanticweb.org/ontologies/2022/2/CDS_V0.6.owl#remedy">
        <rdfs:domain rdf:resource="http://www.semanticweb.org/ontologies/2022/2/CDS_V0.6.owl#Prohibition"/>
        <rdfs:range rdf:resource="http://www.semanticweb.org/ontologies/2022/2/CDS_V0.6.owl#Duty"/>
        <rdfs:comment xml:lang="en">Relates an individual remedy Duty to a Prohibition</rdfs:comment>
    </owl:ObjectProperty>
    


    <!-- http://www.semanticweb.org/ontologies/2022/2/CDS_V0.6.owl#service_link -->


    <owl:ObjectProperty rdf:about="http://www.semanticweb.org/ontologies/2022/2/CDS_V0.6.owl#service_link">
        <rdfs:domain rdf:resource="http://www.semanticweb.org/ontologies/2022/2/CDS_V0.6.owl#Service_Catalogue"/>
        <rdfs:range rdf:resource="http://www.semanticweb.org/ontologies/2022/2/CDS_V0.6.owl#Data_Service"/>
        <rdfs:comment xml:lang="en">A service that is listed in the Catalogue</rdfs:comment>
    </owl:ObjectProperty>
    


    <!-- http://www.semanticweb.org/ontologies/2022/2/CDS_V0.6.owl#sovereign -->


    <owl:ObjectProperty rdf:about="http://www.semanticweb.org/ontologies/2022/2/CDS_V0.6.owl#sovereign">
        <rdfs:domain rdf:resource="http://www.semanticweb.org/ontologies/2022/2/CDS_V0.6.owl#Resource"/>
        <rdfs:range rdf:resource="http://www.semanticweb.org/ontologies/2022/2/CDS_V0.6.owl#Participant"/>
        <rdfs:comment xml:lang="en">The &apos;owner&apos;, i.e. sovereign of the data.</rdfs:comment>
    </owl:ObjectProperty>
    


    <!-- http://www.semanticweb.org/ontologies/2022/2/CDS_V0.6.owl#stores -->


    <owl:ObjectProperty rdf:about="http://www.semanticweb.org/ontologies/2022/2/CDS_V0.6.owl#stores">
        <rdfs:domain rdf:resource="http://www.semanticweb.org/ontologies/2022/2/CDS_V0.6.owl#Clearing_House"/>
        <rdfs:range rdf:resource="http://www.semanticweb.org/ontologies/2022/2/CDS_V0.6.owl#Transaction_Data"/>
        <rdfs:comment xml:lang="en">Information relevant to a transaction (action, service, participant, price) are stored into the Clearing House</rdfs:comment>
    </owl:ObjectProperty>
    


    <!-- http://www.semanticweb.org/ontologies/2022/2/CDS_V0.6.owl#wallet_owner -->


    <owl:ObjectProperty rdf:about="http://www.semanticweb.org/ontologies/2022/2/CDS_V0.6.owl#wallet_owner">
        <rdfs:domain rdf:resource="http://www.semanticweb.org/ontologies/2022/2/CDS_V0.6.owl#Wallet"/>
        <rdfs:range rdf:resource="http://www.semanticweb.org/ontologies/2022/2/CDS_V0.6.owl#Participant"/>
        <rdfs:comment xml:lang="en">Participant associated to a wallet which records his/her transaction and his/her wallet amount.</rdfs:comment>
    </owl:ObjectProperty>
    


    <!-- 
    ///////////////////////////////////////////////////////////////////////////////////////
    //
    // Data properties
    //
    ///////////////////////////////////////////////////////////////////////////////////////
     -->


    


    <!-- http://www.semanticweb.org/ontologies/2022/2/CDS_V0.6.owl#AccessRights -->


    <owl:DatatypeProperty rdf:about="http://www.semanticweb.org/ontologies/2022/2/CDS_V0.6.owl#AccessRights">
        <rdfs:domain rdf:resource="http://www.semanticweb.org/ontologies/2022/2/CDS_V0.6.owl#Data_Service"/>
        <rdfs:domain rdf:resource="http://www.semanticweb.org/ontologies/2022/2/CDS_V0.6.owl#Resource"/>
        <rdfs:range rdf:resource="http://www.w3.org/2001/XMLSchema#string"/>
        <rdfs:comment xml:lang="en">Descriptive information about who can access the item or an indication of its security status</rdfs:comment>
    </owl:DatatypeProperty>
    


    <!-- http://www.semanticweb.org/ontologies/2022/2/CDS_V0.6.owl#Access_Url -->


    <owl:DatatypeProperty rdf:about="http://www.semanticweb.org/ontologies/2022/2/CDS_V0.6.owl#Access_Url">
        <rdfs:domain rdf:resource="http://www.semanticweb.org/ontologies/2022/2/CDS_V0.6.owl#Endpoint"/>
        <rdfs:range rdf:resource="http://www.w3.org/2001/XMLSchema#anyURI"/>
        <rdfs:comment xml:lang="en">Access URL of an endpoint.</rdfs:comment>
    </owl:DatatypeProperty>
    


    <!-- http://www.semanticweb.org/ontologies/2022/2/CDS_V0.6.owl#Action_Identifier -->


    <owl:DatatypeProperty rdf:about="http://www.semanticweb.org/ontologies/2022/2/CDS_V0.6.owl#Action_Identifier">
        <rdfs:domain rdf:resource="http://www.semanticweb.org/ontologies/2022/2/CDS_V0.6.owl#Action"/>
    </owl:DatatypeProperty>
    


    <!-- http://www.semanticweb.org/ontologies/2022/2/CDS_V0.6.owl#BirthDate -->


    <owl:DatatypeProperty rdf:about="http://www.semanticweb.org/ontologies/2022/2/CDS_V0.6.owl#BirthDate">
        <rdfs:domain rdf:resource="http://www.semanticweb.org/ontologies/2022/2/CDS_V0.6.owl#Person"/>
        <rdfs:range rdf:resource="http://www.w3.org/2001/XMLSchema#string"/>
        <rdfs:comment xml:lang="en">Date of birth</rdfs:comment>
    </owl:DatatypeProperty>
    


    <!-- http://www.semanticweb.org/ontologies/2022/2/CDS_V0.6.owl#BirthPlace -->


    <owl:DatatypeProperty rdf:about="http://www.semanticweb.org/ontologies/2022/2/CDS_V0.6.owl#BirthPlace">
        <rdfs:domain rdf:resource="http://www.semanticweb.org/ontologies/2022/2/CDS_V0.6.owl#Person"/>
        <rdfs:range rdf:resource="http://www.w3.org/2001/XMLSchema#string"/>
        <rdfs:comment xml:lang="en">The place where the person was born</rdfs:comment>
    </owl:DatatypeProperty>
    


    <!-- http://www.semanticweb.org/ontologies/2022/2/CDS_V0.6.owl#Byte_size -->


    <owl:DatatypeProperty rdf:about="http://www.semanticweb.org/ontologies/2022/2/CDS_V0.6.owl#Byte_size">
        <rdfs:domain rdf:resource="http://www.semanticweb.org/ontologies/2022/2/CDS_V0.6.owl#Data_Asset"/>
        <rdfs:range rdf:resource="http://www.w3.org/2001/XMLSchema#integer"/>
        <rdfs:comment xml:lang="en">Size of the data asset</rdfs:comment>
    </owl:DatatypeProperty>
    


    <!-- http://www.semanticweb.org/ontologies/2022/2/CDS_V0.6.owl#Category -->


    <owl:DatatypeProperty rdf:about="http://www.semanticweb.org/ontologies/2022/2/CDS_V0.6.owl#Category">
        <rdfs:domain rdf:resource="http://www.semanticweb.org/ontologies/2022/2/CDS_V0.6.owl#Data_Service"/>
        <rdfs:comment xml:lang="en">Category is a tag reporting if the Service is free of charge or not, as defined in the SOW [AD-1].
It can be:
Free / Advanced</rdfs:comment>
    </owl:DatatypeProperty>
    


    <!-- http://www.semanticweb.org/ontologies/2022/2/CDS_V0.6.owl#Certification_Identifier -->


    <owl:DatatypeProperty rdf:about="http://www.semanticweb.org/ontologies/2022/2/CDS_V0.6.owl#Certification_Identifier">
        <rdfs:domain rdf:resource="http://www.semanticweb.org/ontologies/2022/2/CDS_V0.6.owl#Certification"/>
        <rdfs:range rdf:resource="http://www.w3.org/2001/XMLSchema#string"/>
        <rdfs:comment xml:lang="en">Identifier of the Certification</rdfs:comment>
    </owl:DatatypeProperty>
    


    <!-- http://www.semanticweb.org/ontologies/2022/2/CDS_V0.6.owl#Checksum -->


    <owl:DatatypeProperty rdf:about="http://www.semanticweb.org/ontologies/2022/2/CDS_V0.6.owl#Checksum">
        <rdfs:domain rdf:resource="http://www.semanticweb.org/ontologies/2022/2/CDS_V0.6.owl#Data_Asset"/>
        <rdfs:comment xml:lang="en">Checksum of the data asset</rdfs:comment>
    </owl:DatatypeProperty>
    


    <!-- http://www.semanticweb.org/ontologies/2022/2/CDS_V0.6.owl#Clearing_House_Homepage -->


    <owl:DatatypeProperty rdf:about="http://www.semanticweb.org/ontologies/2022/2/CDS_V0.6.owl#Clearing_House_Homepage">
        <rdfs:domain rdf:resource="http://www.semanticweb.org/ontologies/2022/2/CDS_V0.6.owl#Clearing_House"/>
        <rdfs:range rdf:resource="http://www.w3.org/2001/XMLSchema#anyURI"/>
        <rdfs:comment xml:lang="en">A homepage of the Clearing House.</rdfs:comment>
    </owl:DatatypeProperty>
    


    <!-- http://www.semanticweb.org/ontologies/2022/2/CDS_V0.6.owl#Clearing_House_curator -->


    <owl:DatatypeProperty rdf:about="http://www.semanticweb.org/ontologies/2022/2/CDS_V0.6.owl#Clearing_House_curator">
        <rdfs:domain rdf:resource="http://www.semanticweb.org/ontologies/2022/2/CDS_V0.6.owl#Clearing_House"/>
        <rdfs:range rdf:resource="http://www.w3.org/2001/XMLSchema#string"/>
        <rdfs:comment xml:lang="en">Participant responsible for technical maintenance of the Ecosystem Component.</rdfs:comment>
    </owl:DatatypeProperty>
    


    <!-- http://www.semanticweb.org/ontologies/2022/2/CDS_V0.6.owl#Clearing_House_maintainer -->


    <owl:DatatypeProperty rdf:about="http://www.semanticweb.org/ontologies/2022/2/CDS_V0.6.owl#Clearing_House_maintainer">
        <rdfs:domain rdf:resource="http://www.semanticweb.org/ontologies/2022/2/CDS_V0.6.owl#Clearing_House"/>
        <rdfs:range rdf:resource="http://www.w3.org/2001/XMLSchema#string"/>
        <rdfs:comment xml:lang="en">Descriptive information on the Participant responsible for the correctness of the content offered by the Ecosystem Component.</rdfs:comment>
    </owl:DatatypeProperty>
    


    <!-- http://www.semanticweb.org/ontologies/2022/2/CDS_V0.6.owl#Component_Certification_Level -->


    <owl:DatatypeProperty rdf:about="http://www.semanticweb.org/ontologies/2022/2/CDS_V0.6.owl#Component_Certification_Level">
        <rdfs:domain rdf:resource="http://www.semanticweb.org/ontologies/2022/2/CDS_V0.6.owl#Component_Certification"/>
        <rdfs:range rdf:resource="http://www.w3.org/2001/XMLSchema#string"/>
        <rdfs:comment xml:lang="en">Certification issued for the given Ecosystem Component</rdfs:comment>
    </owl:DatatypeProperty>
    


    <!-- http://www.semanticweb.org/ontologies/2022/2/CDS_V0.6.owl#Configuration_model_log_level -->


    <owl:DatatypeProperty rdf:about="http://www.semanticweb.org/ontologies/2022/2/CDS_V0.6.owl#Configuration_model_log_level">
        <rdfs:domain rdf:resource="http://www.semanticweb.org/ontologies/2022/2/CDS_V0.6.owl#Connector"/>
        <rdfs:range rdf:resource="http://www.w3.org/2001/XMLSchema#string"/>
        <rdfs:comment xml:lang="en">Debug, minimal logging, no logging</rdfs:comment>
    </owl:DatatypeProperty>
    


    <!-- http://www.semanticweb.org/ontologies/2022/2/CDS_V0.6.owl#ConformsTo -->


    <owl:DatatypeProperty rdf:about="http://www.semanticweb.org/ontologies/2022/2/CDS_V0.6.owl#ConformsTo">
        <rdfs:domain rdf:resource="http://www.semanticweb.org/ontologies/2022/2/CDS_V0.6.owl#Data_Service"/>
        <rdfs:domain rdf:resource="http://www.semanticweb.org/ontologies/2022/2/CDS_V0.6.owl#Resource"/>
        <rdfs:range rdf:resource="http://www.w3.org/2001/XMLSchema#string"/>
        <rdfs:comment xml:lang="en">An established standard to which the described item conforms.</rdfs:comment>
    </owl:DatatypeProperty>
    


    <!-- http://www.semanticweb.org/ontologies/2022/2/CDS_V0.6.owl#Connector_Deploy_Mode -->


    <owl:DatatypeProperty rdf:about="http://www.semanticweb.org/ontologies/2022/2/CDS_V0.6.owl#Connector_Deploy_Mode">
        <rdfs:domain rdf:resource="http://www.semanticweb.org/ontologies/2022/2/CDS_V0.6.owl#Connector"/>
        <rdfs:range rdf:resource="http://www.w3.org/2001/XMLSchema#string"/>
        <rdfs:comment xml:lang="en">Deploy mode of a Connector.
Production or test.</rdfs:comment>
    </owl:DatatypeProperty>
    


    <!-- http://www.semanticweb.org/ontologies/2022/2/CDS_V0.6.owl#Connector_Identifier -->


    <owl:DatatypeProperty rdf:about="http://www.semanticweb.org/ontologies/2022/2/CDS_V0.6.owl#Connector_Identifier">
        <rdfs:domain rdf:resource="http://www.semanticweb.org/ontologies/2022/2/CDS_V0.6.owl#Connector"/>
        <rdfs:range rdf:resource="http://www.w3.org/2001/XMLSchema#string"/>
        <rdfs:comment xml:lang="en">Identifier of the Connector</rdfs:comment>
    </owl:DatatypeProperty>
    


    <!-- http://www.semanticweb.org/ontologies/2022/2/CDS_V0.6.owl#Connector_Status -->


    <owl:DatatypeProperty rdf:about="http://www.semanticweb.org/ontologies/2022/2/CDS_V0.6.owl#Connector_Status">
        <rdfs:domain rdf:resource="http://www.semanticweb.org/ontologies/2022/2/CDS_V0.6.owl#Connector"/>
        <rdfs:range rdf:resource="http://www.w3.org/2001/XMLSchema#string"/>
        <rdfs:comment xml:lang="en">Offline, online, badly configured</rdfs:comment>
    </owl:DatatypeProperty>
    


    <!-- http://www.semanticweb.org/ontologies/2022/2/CDS_V0.6.owl#Connector_curator -->


    <owl:DatatypeProperty rdf:about="http://www.semanticweb.org/ontologies/2022/2/CDS_V0.6.owl#Connector_curator">
        <rdfs:domain rdf:resource="http://www.semanticweb.org/ontologies/2022/2/CDS_V0.6.owl#Connector"/>
        <rdfs:range rdf:resource="http://www.w3.org/2001/XMLSchema#string"/>
        <rdfs:comment xml:lang="en">Descriptive information on the Participant responsible for technical maintenance of the Ecosystem Component.</rdfs:comment>
    </owl:DatatypeProperty>
    


    <!-- http://www.semanticweb.org/ontologies/2022/2/CDS_V0.6.owl#Connector_description -->


    <owl:DatatypeProperty rdf:about="http://www.semanticweb.org/ontologies/2022/2/CDS_V0.6.owl#Connector_description">
        <rdfs:domain rdf:resource="http://www.semanticweb.org/ontologies/2022/2/CDS_V0.6.owl#Connector"/>
        <rdfs:range rdf:resource="http://www.w3.org/2001/XMLSchema#string"/>
        <rdfs:comment xml:lang="en">References to Connector which is deployed / maintained in the Configuration model</rdfs:comment>
    </owl:DatatypeProperty>
    


    <!-- http://www.semanticweb.org/ontologies/2022/2/CDS_V0.6.owl#Connector_maintainer -->


    <owl:DatatypeProperty rdf:about="http://www.semanticweb.org/ontologies/2022/2/CDS_V0.6.owl#Connector_maintainer">
        <rdfs:domain rdf:resource="http://www.semanticweb.org/ontologies/2022/2/CDS_V0.6.owl#Connector"/>
        <rdfs:range rdf:resource="http://www.w3.org/2001/XMLSchema#string"/>
        <rdfs:comment xml:lang="en">Descriptive information on the Participant responsible for the correctness of the content offered by the Ecosystem Component.</rdfs:comment>
    </owl:DatatypeProperty>
    


    <!-- http://www.semanticweb.org/ontologies/2022/2/CDS_V0.6.owl#Constraint_Identifier -->


    <owl:DatatypeProperty rdf:about="http://www.semanticweb.org/ontologies/2022/2/CDS_V0.6.owl#Constraint_Identifier">
        <rdfs:domain rdf:resource="http://www.semanticweb.org/ontologies/2022/2/CDS_V0.6.owl#Constraint"/>
        <rdfs:range rdf:resource="http://www.w3.org/2001/XMLSchema#string"/>
        <rdfs:comment xml:lang="en">Identifier of the Constraints</rdfs:comment>
    </owl:DatatypeProperty>
    


    <!-- http://www.semanticweb.org/ontologies/2022/2/CDS_V0.6.owl#Constraints -->


    <owl:DatatypeProperty rdf:about="http://www.semanticweb.org/ontologies/2022/2/CDS_V0.6.owl#Constraints">
        <rdfs:domain rdf:resource="http://www.semanticweb.org/ontologies/2022/2/CDS_V0.6.owl#Transaction_Data"/>
        <rdfs:comment xml:lang="en">Descriptive information on the (potential) constraints associated to the access interface</rdfs:comment>
    </owl:DatatypeProperty>
    


    <!-- http://www.semanticweb.org/ontologies/2022/2/CDS_V0.6.owl#ContactPoint -->


    <owl:DatatypeProperty rdf:about="http://www.semanticweb.org/ontologies/2022/2/CDS_V0.6.owl#ContactPoint">
        <rdfs:domain rdf:resource="http://www.semanticweb.org/ontologies/2022/2/CDS_V0.6.owl#Service_Catalogue"/>
        <rdfs:range rdf:resource="http://www.w3.org/2001/XMLSchema#string"/>
        <rdfs:comment xml:lang="en">Relevant contact information for the cataloged item</rdfs:comment>
    </owl:DatatypeProperty>
    


    <!-- http://www.semanticweb.org/ontologies/2022/2/CDS_V0.6.owl#Content_Provenance -->


    <owl:DatatypeProperty rdf:about="http://www.semanticweb.org/ontologies/2022/2/CDS_V0.6.owl#Content_Provenance">
        <rdfs:domain rdf:resource="http://www.semanticweb.org/ontologies/2022/2/CDS_V0.6.owl#Broker"/>
        <rdfs:domain rdf:resource="http://www.semanticweb.org/ontologies/2022/2/CDS_V0.6.owl#Resource"/>
        <rdfs:range rdf:resource="http://www.w3.org/2001/XMLSchema#string"/>
        <rdfs:comment xml:lang="en">Origin of the Content</rdfs:comment>
    </owl:DatatypeProperty>
    


    <!-- http://www.semanticweb.org/ontologies/2022/2/CDS_V0.6.owl#Content_standard -->


    <owl:DatatypeProperty rdf:about="http://www.semanticweb.org/ontologies/2022/2/CDS_V0.6.owl#Content_standard">
        <rdfs:domain rdf:resource="http://www.semanticweb.org/ontologies/2022/2/CDS_V0.6.owl#Digital_Content"/>
        <rdfs:range rdf:resource="http://www.w3.org/2001/XMLSchema#anyURI"/>
        <rdfs:comment xml:lang="en">IRI containing document, which defines the standard for the given Digital Content. The content is assumed to conform to that Standard.</rdfs:comment>
    </owl:DatatypeProperty>
    


    <!-- http://www.semanticweb.org/ontologies/2022/2/CDS_V0.6.owl#Context -->


    <owl:DatatypeProperty rdf:about="http://www.semanticweb.org/ontologies/2022/2/CDS_V0.6.owl#Context">
        <rdfs:domain rdf:resource="http://www.semanticweb.org/ontologies/2022/2/CDS_V0.6.owl#Participant"/>
        <rdfs:range rdf:resource="http://www.w3.org/2001/XMLSchema#string"/>
        <rdfs:comment xml:lang="en">Legal,
Commercial,
Technical,
Business,
Federative</rdfs:comment>
    </owl:DatatypeProperty>
    


    <!-- http://www.semanticweb.org/ontologies/2022/2/CDS_V0.6.owl#ContractOfferRef -->


    <owl:DatatypeProperty rdf:about="http://www.semanticweb.org/ontologies/2022/2/CDS_V0.6.owl#ContractOfferRef">
        <rdfs:domain rdf:resource="http://www.semanticweb.org/ontologies/2022/2/CDS_V0.6.owl#Resource"/>
        <rdfs:range rdf:resource="http://www.w3.org/2001/XMLSchema#string"/>
        <dc:contributor xml:lang="en">Reference to a Contract Offer defining the authorized use of the Resource.</dc:contributor>
    </owl:DatatypeProperty>
    


    <!-- http://www.semanticweb.org/ontologies/2022/2/CDS_V0.6.owl#Contract_Identifier -->


    <owl:DatatypeProperty rdf:about="http://www.semanticweb.org/ontologies/2022/2/CDS_V0.6.owl#Contract_Identifier">
        <rdfs:domain rdf:resource="http://www.semanticweb.org/ontologies/2022/2/CDS_V0.6.owl#Contract"/>
        <rdfs:range rdf:resource="http://www.w3.org/2001/XMLSchema#string"/>
        <rdfs:comment xml:lang="en">Unambiguous identifier to identify the Contract</rdfs:comment>
    </owl:DatatypeProperty>
    


    <!-- http://www.semanticweb.org/ontologies/2022/2/CDS_V0.6.owl#Contract_date -->


    <owl:DatatypeProperty rdf:about="http://www.semanticweb.org/ontologies/2022/2/CDS_V0.6.owl#Contract_date">
        <rdfs:domain rdf:resource="http://www.semanticweb.org/ontologies/2022/2/CDS_V0.6.owl#Contract"/>
        <rdfs:range rdf:resource="http://www.w3.org/2001/XMLSchema#dateTimeStamp"/>
        <rdfs:comment xml:lang="en">Absolute datetime of signing the Contract</rdfs:comment>
    </owl:DatatypeProperty>
    


    <!-- http://www.semanticweb.org/ontologies/2022/2/CDS_V0.6.owl#Contract_end -->


    <owl:DatatypeProperty rdf:about="http://www.semanticweb.org/ontologies/2022/2/CDS_V0.6.owl#Contract_end">
        <rdfs:domain rdf:resource="http://www.semanticweb.org/ontologies/2022/2/CDS_V0.6.owl#Contract"/>
        <rdfs:range rdf:resource="http://www.w3.org/2001/XMLSchema#dateTimeStamp"/>
        <rdfs:comment xml:lang="en">Absolute datetime the Contract is requested, offered or expected to end. If omitted, the contract has to be explicitly terminated by any of the parties.</rdfs:comment>
    </owl:DatatypeProperty>
    


    <!-- http://www.semanticweb.org/ontologies/2022/2/CDS_V0.6.owl#Contract_start -->


    <owl:DatatypeProperty rdf:about="http://www.semanticweb.org/ontologies/2022/2/CDS_V0.6.owl#Contract_start">
        <rdfs:domain rdf:resource="http://www.semanticweb.org/ontologies/2022/2/CDS_V0.6.owl#Contract"/>
        <rdfs:range rdf:resource="http://www.w3.org/2001/XMLSchema#dateTimeStamp"/>
        <rdfs:comment xml:lang="en">Absolute datetime the Contract is requested, offered or expected to start, depending on the type of Contract.</rdfs:comment>
    </owl:DatatypeProperty>
    


    <!-- http://www.semanticweb.org/ontologies/2022/2/CDS_V0.6.owl#Cost_Centre -->


    <owl:DatatypeProperty rdf:about="http://www.semanticweb.org/ontologies/2022/2/CDS_V0.6.owl#Cost_Centre">
        <rdfs:domain rdf:resource="http://www.semanticweb.org/ontologies/2022/2/CDS_V0.6.owl#Data_Service"/>
        <rdfs:range rdf:resource="http://www.w3.org/2001/XMLSchema#string"/>
        <rdfs:comment xml:lang="en">Business unit that is only responsible for the costs that incurs</rdfs:comment>
    </owl:DatatypeProperty>
    


    <!-- http://www.semanticweb.org/ontologies/2022/2/CDS_V0.6.owl#Cost_model -->


    <owl:DatatypeProperty rdf:about="http://www.semanticweb.org/ontologies/2022/2/CDS_V0.6.owl#Cost_model">
        <rdfs:domain rdf:resource="http://www.semanticweb.org/ontologies/2022/2/CDS_V0.6.owl#Transaction_Data"/>
        <rdfs:range rdf:resource="http://www.w3.org/2001/XMLSchema#string"/>
        <rdfs:comment xml:lang="en">Description of the cost model approach applied to the available interface</rdfs:comment>
    </owl:DatatypeProperty>
    


    <!-- http://www.semanticweb.org/ontologies/2022/2/CDS_V0.6.owl#Country -->


    <owl:DatatypeProperty rdf:about="http://www.semanticweb.org/ontologies/2022/2/CDS_V0.6.owl#Country">
        <rdfs:domain rdf:resource="http://www.semanticweb.org/ontologies/2022/2/CDS_V0.6.owl#Person"/>
        <rdfs:range rdf:resource="http://www.w3.org/2001/XMLSchema#string"/>
        <rdfs:comment xml:lang="en">Nationality of the person</rdfs:comment>
    </owl:DatatypeProperty>
    


    <!-- http://www.semanticweb.org/ontologies/2022/2/CDS_V0.6.owl#DataAppVersion -->


    <owl:DatatypeProperty rdf:about="http://www.semanticweb.org/ontologies/2022/2/CDS_V0.6.owl#DataAppVersion">
        <rdfs:domain rdf:resource="http://www.semanticweb.org/ontologies/2022/2/CDS_V0.6.owl#Data_App"/>
        <rdfs:range rdf:resource="http://www.w3.org/2001/XMLSchema#integer"/>
        <rdfs:comment xml:lang="en">Version of the installed application</rdfs:comment>
    </owl:DatatypeProperty>
    


    <!-- http://www.semanticweb.org/ontologies/2022/2/CDS_V0.6.owl#Data_App_Functionality -->


    <owl:DatatypeProperty rdf:about="http://www.semanticweb.org/ontologies/2022/2/CDS_V0.6.owl#Data_App_Functionality">
        <rdfs:domain rdf:resource="http://www.semanticweb.org/ontologies/2022/2/CDS_V0.6.owl#Data_App"/>
        <rdfs:range rdf:resource="http://www.w3.org/2001/XMLSchema#string"/>
        <rdfs:comment xml:lang="en">Description of the capability of a Data App to handle a type of data in a particular way</rdfs:comment>
    </owl:DatatypeProperty>
    


    <!-- http://www.semanticweb.org/ontologies/2022/2/CDS_V0.6.owl#Data_Service_Identifier -->


    <owl:DatatypeProperty rdf:about="http://www.semanticweb.org/ontologies/2022/2/CDS_V0.6.owl#Data_Service_Identifier">
        <rdfs:domain rdf:resource="http://www.semanticweb.org/ontologies/2022/2/CDS_V0.6.owl#Data_Service"/>
        <rdfs:range rdf:resource="http://www.w3.org/2001/XMLSchema#string"/>
        <rdfs:comment xml:lang="en">Unique identifier of the Service</rdfs:comment>
    </owl:DatatypeProperty>
    


    <!-- http://www.semanticweb.org/ontologies/2022/2/CDS_V0.6.owl#Data_Service_Type -->


    <owl:DatatypeProperty rdf:about="http://www.semanticweb.org/ontologies/2022/2/CDS_V0.6.owl#Data_Service_Type">
        <rdfs:domain rdf:resource="http://www.semanticweb.org/ontologies/2022/2/CDS_V0.6.owl#Data_Service"/>
        <rdfs:range rdf:resource="http://www.w3.org/2001/XMLSchema#string"/>
        <rdfs:comment xml:lang="en">Type of operation which characterised the scope and kind of Service. 
Possible values: discovery, download, trace, distribute, produce, process, order, archive, transform, view, other.</rdfs:comment>
    </owl:DatatypeProperty>
    


    <!-- http://www.semanticweb.org/ontologies/2022/2/CDS_V0.6.owl#Data_Service_Url -->


    <owl:DatatypeProperty rdf:about="http://www.semanticweb.org/ontologies/2022/2/CDS_V0.6.owl#Data_Service_Url">
        <rdfs:domain rdf:resource="http://www.semanticweb.org/ontologies/2022/2/CDS_V0.6.owl#Data_Service"/>
        <rdfs:range rdf:resource="http://www.w3.org/2001/XMLSchema#anyURI"/>
        <rdfs:comment xml:lang="en">URL of the Data Service webpage that replaces the Internet Protocol (IP) address.</rdfs:comment>
    </owl:DatatypeProperty>
    


    <!-- http://www.semanticweb.org/ontologies/2022/2/CDS_V0.6.owl#Deployment_option -->


    <owl:DatatypeProperty rdf:about="http://www.semanticweb.org/ontologies/2022/2/CDS_V0.6.owl#Deployment_option">
        <rdfs:domain rdf:resource="http://www.semanticweb.org/ontologies/2022/2/CDS_V0.6.owl#Data_App"/>
        <rdfs:range rdf:resource="http://www.w3.org/2001/XMLSchema#string"/>
        <rdfs:comment xml:lang="en">On-premises installation: A Service Provider deploys the Data App inside of an on-premises CDS Connector on behalf of the Data Provider. This is assumed to be the default case.

On-premises injection: A Service Provider deploys the Data App inside of an on-premises CDS Connector on behalf of the Data Consumer (asking for customized data preprocessing, according to contract specifications; e.g., edge computing).  

Remote integration: A Service Provider integrates a remote Data App service on behalf of the Data Provider. In this scenario, the Data App is hosted by different participants and used remotely.</rdfs:comment>
    </owl:DatatypeProperty>
    


    <!-- http://www.semanticweb.org/ontologies/2022/2/CDS_V0.6.owl#EmailAddress -->


    <owl:DatatypeProperty rdf:about="http://www.semanticweb.org/ontologies/2022/2/CDS_V0.6.owl#EmailAddress">
        <rdfs:domain rdf:resource="http://www.semanticweb.org/ontologies/2022/2/CDS_V0.6.owl#Person"/>
        <rdfs:range rdf:resource="http://www.w3.org/2001/XMLSchema#string"/>
        <rdfs:comment xml:lang="en">Email Address of the Person</rdfs:comment>
    </owl:DatatypeProperty>
    


    <!-- http://www.semanticweb.org/ontologies/2022/2/CDS_V0.6.owl#Endpoint_documentation -->


    <owl:DatatypeProperty rdf:about="http://www.semanticweb.org/ontologies/2022/2/CDS_V0.6.owl#Endpoint_documentation">
        <rdfs:domain rdf:resource="http://www.semanticweb.org/ontologies/2022/2/CDS_V0.6.owl#Endpoint"/>
        <rdfs:range rdf:resource="http://www.w3.org/2001/XMLSchema#anyURI"/>
        <rdfs:comment xml:lang="en">IRI reference to a documentation of the endpoint, e.g., reference to an OpenAPI-based documentation.</rdfs:comment>
    </owl:DatatypeProperty>
    


    <!-- http://www.semanticweb.org/ontologies/2022/2/CDS_V0.6.owl#Endpoint_information -->


    <owl:DatatypeProperty rdf:about="http://www.semanticweb.org/ontologies/2022/2/CDS_V0.6.owl#Endpoint_information">
        <rdfs:domain rdf:resource="http://www.semanticweb.org/ontologies/2022/2/CDS_V0.6.owl#Endpoint"/>
        <rdfs:range rdf:resource="http://www.w3.org/2001/XMLSchema#string"/>
        <rdfs:comment xml:lang="en">Human-readable information and description of the endpoint.</rdfs:comment>
    </owl:DatatypeProperty>
    


    <!-- http://www.semanticweb.org/ontologies/2022/2/CDS_V0.6.owl#Evaluation_facility -->


    <owl:DatatypeProperty rdf:about="http://www.semanticweb.org/ontologies/2022/2/CDS_V0.6.owl#Evaluation_facility">
        <rdfs:domain rdf:resource="http://www.semanticweb.org/ontologies/2022/2/CDS_V0.6.owl#Certification"/>
        <rdfs:comment xml:lang="en">Evaluation Facility that performed and issued given Certification.</rdfs:comment>
    </owl:DatatypeProperty>
    


    <!-- http://www.semanticweb.org/ontologies/2022/2/CDS_V0.6.owl#Function -->


    <owl:DatatypeProperty rdf:about="http://www.semanticweb.org/ontologies/2022/2/CDS_V0.6.owl#Function">
        <rdfs:domain rdf:resource="http://www.semanticweb.org/ontologies/2022/2/CDS_V0.6.owl#Participant"/>
        <rdfs:range rdf:resource="http://www.w3.org/2001/XMLSchema#string"/>
        <rdfs:comment xml:lang="en">Legally owns data and offers this for consumption 

Provides data on the behalf of an owner and may be the Customer of a Service Provider as well.

Directly manages and operates resources aimed at data distribution. 

Single user, organization or industry which consumes data to make own business and maintain a business relationship with the Service Provider. Service Consumers can also be Service Providers if they provide other consumers with a service.

Users belonging to a Federation, that have access to free services thanks to credentials managed by the Federated Identity Providers</rdfs:comment>
    </owl:DatatypeProperty>
    


    <!-- http://www.semanticweb.org/ontologies/2022/2/CDS_V0.6.owl#Identity -->


    <owl:DatatypeProperty rdf:about="http://www.semanticweb.org/ontologies/2022/2/CDS_V0.6.owl#Identity">
        <rdfs:domain rdf:resource="http://www.semanticweb.org/ontologies/2022/2/CDS_V0.6.owl#Participant"/>
        <rdfs:comment xml:lang="en">Every participant is given a unique identity by the Identity Provider. 

By default, and in accordance with linked-data principles, a participant can unambiguously be identified by a dereferencable HTTPS URL, which references to a live metadata document describing the participant. This identity is confirmed by a certificate.</rdfs:comment>
    </owl:DatatypeProperty>
    


    <!-- http://www.semanticweb.org/ontologies/2022/2/CDS_V0.6.owl#Identity_Provider_curator -->


    <owl:DatatypeProperty rdf:about="http://www.semanticweb.org/ontologies/2022/2/CDS_V0.6.owl#Identity_Provider_curator">
        <rdfs:domain rdf:resource="http://www.semanticweb.org/ontologies/2022/2/CDS_V0.6.owl#Identity_Provider"/>
        <rdfs:range rdf:resource="http://www.w3.org/2001/XMLSchema#string"/>
        <rdfs:comment xml:lang="en">Participant responsible for technical maintenance of the Ecosystem Component.</rdfs:comment>
    </owl:DatatypeProperty>
    


    <!-- http://www.semanticweb.org/ontologies/2022/2/CDS_V0.6.owl#Identity_Provider_maintainer -->


    <owl:DatatypeProperty rdf:about="http://www.semanticweb.org/ontologies/2022/2/CDS_V0.6.owl#Identity_Provider_maintainer">
        <rdfs:domain rdf:resource="http://www.semanticweb.org/ontologies/2022/2/CDS_V0.6.owl#Identity_Provider"/>
        <rdfs:range rdf:resource="http://www.w3.org/2001/XMLSchema#string"/>
        <rdfs:comment xml:lang="en">Descriptive information on the Participant responsible for the correctness of the content offered by the Ecosystem Component.</rdfs:comment>
    </owl:DatatypeProperty>
    


    <!-- http://www.semanticweb.org/ontologies/2022/2/CDS_V0.6.owl#Inbound_model_version -->


    <owl:DatatypeProperty rdf:about="http://www.semanticweb.org/ontologies/2022/2/CDS_V0.6.owl#Inbound_model_version">
        <rdfs:domain rdf:resource="http://www.semanticweb.org/ontologies/2022/2/CDS_V0.6.owl#Ecosystem_Component"/>
        <rdfs:range rdf:resource="http://www.w3.org/2001/XMLSchema#string"/>
        <rdfs:comment xml:lang="en">Information Model version that the Ecosystem Component is capable of reading/processing.</rdfs:comment>
    </owl:DatatypeProperty>
    


    <!-- http://www.semanticweb.org/ontologies/2022/2/CDS_V0.6.owl#Inbound_topic -->


    <owl:DatatypeProperty rdf:about="http://www.semanticweb.org/ontologies/2022/2/CDS_V0.6.owl#Inbound_topic">
        <rdfs:domain rdf:resource="http://www.semanticweb.org/ontologies/2022/2/CDS_V0.6.owl#Endpoint"/>
        <rdfs:range rdf:resource="http://www.w3.org/2001/XMLSchema#string"/>
        <rdfs:comment xml:lang="en">Relative path used for inbound communication via this endpoint, i.e. input messages and faults only.</rdfs:comment>
    </owl:DatatypeProperty>
    


    <!-- http://www.semanticweb.org/ontologies/2022/2/CDS_V0.6.owl#ItemModificationDate -->


    <owl:DatatypeProperty rdf:about="http://www.semanticweb.org/ontologies/2022/2/CDS_V0.6.owl#ItemModificationDate">
        <rdfs:domain rdf:resource="http://www.semanticweb.org/ontologies/2022/2/CDS_V0.6.owl#Service_Catalogue"/>
        <rdfs:range rdf:resource="http://www.w3.org/2001/XMLSchema#string"/>
        <rdfs:comment xml:lang="en">Most recent date on which the item was changed, updated or modified.</rdfs:comment>
    </owl:DatatypeProperty>
    


    <!-- http://www.semanticweb.org/ontologies/2022/2/CDS_V0.6.owl#ItemPublicationDate -->


    <owl:DatatypeProperty rdf:about="http://www.semanticweb.org/ontologies/2022/2/CDS_V0.6.owl#ItemPublicationDate">
        <rdfs:domain rdf:resource="http://www.semanticweb.org/ontologies/2022/2/CDS_V0.6.owl#Service_Catalogue"/>
        <rdfs:range rdf:resource="http://www.w3.org/2001/XMLSchema#string"/>
        <rdfs:comment xml:lang="en">Date of formal issuance (e.g., publication) of the item.</rdfs:comment>
    </owl:DatatypeProperty>
    


    <!-- http://www.semanticweb.org/ontologies/2022/2/CDS_V0.6.owl#Keyword -->


    <owl:DatatypeProperty rdf:about="http://www.semanticweb.org/ontologies/2022/2/CDS_V0.6.owl#Keyword">
        <rdfs:domain rdf:resource="http://www.semanticweb.org/ontologies/2022/2/CDS_V0.6.owl#Digital_Content"/>
        <rdfs:range rdf:resource="http://www.w3.org/2001/XMLSchema#string"/>
        <rdfs:comment xml:lang="en">Controlled keywords that describe the nature, purpose, or use of the content.
Possible keyword:
numeric, text, still image, geospatial, audio, video, software, interactive resource, 3D, other.
Possible examples: numeric, text, still image, geospatial, audio, video, software, interactive resource,  3D, other.</rdfs:comment>
    </owl:DatatypeProperty>
    


    <!-- http://www.semanticweb.org/ontologies/2022/2/CDS_V0.6.owl#Language -->


    <owl:DatatypeProperty rdf:about="http://www.semanticweb.org/ontologies/2022/2/CDS_V0.6.owl#Language">
        <rdfs:domain rdf:resource="http://www.semanticweb.org/ontologies/2022/2/CDS_V0.6.owl#Resource"/>
        <rdfs:range rdf:resource="http://www.w3.org/2001/XMLSchema#string"/>
        <dc:contributor xml:lang="en">Language of the item.</dc:contributor>
    </owl:DatatypeProperty>
    


    <!-- http://www.semanticweb.org/ontologies/2022/2/CDS_V0.6.owl#Last_valid_date -->


    <owl:DatatypeProperty rdf:about="http://www.semanticweb.org/ontologies/2022/2/CDS_V0.6.owl#Last_valid_date">
        <rdfs:domain rdf:resource="http://www.semanticweb.org/ontologies/2022/2/CDS_V0.6.owl#Certification"/>
        <rdfs:range rdf:resource="http://www.w3.org/2001/XMLSchema#dateTimeStamp"/>
        <rdfs:comment xml:lang="en">Last date the given Certification is considered valid</rdfs:comment>
    </owl:DatatypeProperty>
    


    <!-- http://www.semanticweb.org/ontologies/2022/2/CDS_V0.6.owl#License -->


    <owl:DatatypeProperty rdf:about="http://www.semanticweb.org/ontologies/2022/2/CDS_V0.6.owl#License">
        <rdfs:domain rdf:resource="http://www.semanticweb.org/ontologies/2022/2/CDS_V0.6.owl#Data_Service"/>
        <rdfs:domain rdf:resource="http://www.semanticweb.org/ontologies/2022/2/CDS_V0.6.owl#Resource"/>
        <rdfs:range rdf:resource="http://www.w3.org/2001/XMLSchema#anyURI"/>
        <rdfs:comment xml:lang="en">Reference to a legal document under which the resource is made available</rdfs:comment>
    </owl:DatatypeProperty>
    


    <!-- http://www.semanticweb.org/ontologies/2022/2/CDS_V0.6.owl#Logical_Constraint_Identifier -->


    <owl:DatatypeProperty rdf:about="http://www.semanticweb.org/ontologies/2022/2/CDS_V0.6.owl#Logical_Constraint_Identifier">
        <rdfs:domain rdf:resource="http://www.semanticweb.org/ontologies/2022/2/CDS_V0.6.owl#Logical_Constraint"/>
        <rdfs:range rdf:resource="http://www.w3.org/2001/XMLSchema#string"/>
        <rdfs:comment xml:lang="en">Identifier of the Logical Constraint</rdfs:comment>
    </owl:DatatypeProperty>
    


    <!-- http://www.semanticweb.org/ontologies/2022/2/CDS_V0.6.owl#Membership_end -->


    <owl:DatatypeProperty rdf:about="http://www.semanticweb.org/ontologies/2022/2/CDS_V0.6.owl#Membership_end">
        <rdfs:domain rdf:resource="http://www.semanticweb.org/ontologies/2022/2/CDS_V0.6.owl#Participant_Certification"/>
        <rdfs:range rdf:resource="http://www.w3.org/2001/XMLSchema#dateTimeStamp"/>
        <rdfs:comment xml:lang="en">End of the Participant’s CDS Membership.</rdfs:comment>
    </owl:DatatypeProperty>
    


    <!-- http://www.semanticweb.org/ontologies/2022/2/CDS_V0.6.owl#ModificationDate -->


    <owl:DatatypeProperty rdf:about="http://www.semanticweb.org/ontologies/2022/2/CDS_V0.6.owl#ModificationDate">
        <rdfs:domain rdf:resource="http://www.semanticweb.org/ontologies/2022/2/CDS_V0.6.owl#Data_Asset"/>
        <rdfs:range rdf:resource="http://www.w3.org/2001/XMLSchema#string"/>
        <rdfs:comment xml:lang="en">Most recent date on which the data asset was changed, updated or modified.</rdfs:comment>
    </owl:DatatypeProperty>
    


    <!-- http://www.semanticweb.org/ontologies/2022/2/CDS_V0.6.owl#Name -->


    <owl:DatatypeProperty rdf:about="http://www.semanticweb.org/ontologies/2022/2/CDS_V0.6.owl#Name">
        <rdfs:domain rdf:resource="http://www.semanticweb.org/ontologies/2022/2/CDS_V0.6.owl#Person"/>
        <rdfs:range rdf:resource="http://www.w3.org/2001/XMLSchema#string"/>
        <rdfs:comment xml:lang="en">Name of the Person</rdfs:comment>
    </owl:DatatypeProperty>
    


    <!-- http://www.semanticweb.org/ontologies/2022/2/CDS_V0.6.owl#Objective -->


    <owl:DatatypeProperty rdf:about="http://www.semanticweb.org/ontologies/2022/2/CDS_V0.6.owl#Objective">
        <rdfs:domain rdf:resource="http://www.semanticweb.org/ontologies/2022/2/CDS_V0.6.owl#Participant"/>
        <rdfs:range rdf:resource="http://www.w3.org/2001/XMLSchema#string"/>
        <rdfs:comment xml:lang="en">Data sovereignty,
Data commissioning or
Decommissioning,
Data distribution,
Data exploitation,
Data usage policies,
Collaboration</rdfs:comment>
    </owl:DatatypeProperty>
    


    <!-- http://www.semanticweb.org/ontologies/2022/2/CDS_V0.6.owl#Operand -->


    <owl:DatatypeProperty rdf:about="http://www.semanticweb.org/ontologies/2022/2/CDS_V0.6.owl#Operand">
        <rdfs:domain rdf:resource="http://www.semanticweb.org/ontologies/2022/2/CDS_V0.6.owl#Logical_Constraint"/>
        <rdfs:range rdf:resource="http://www.w3.org/2001/XMLSchema#string"/>
        <rdfs:comment xml:lang="en">Operand is an abstract property for a logical relationship.
Possible values:
AND: The relation is satisfied when all of the Constraints are satisfied.
ANDSEQUENCE: The relation is satisfied when each of the Constraints are satisfied in the order specified.
OR: The relation is satisfied when at least one of the Constraints is satisfied.
XONE (only one): The relation is satisfied when only one, and not more, of the Constaints is satisfied</rdfs:comment>
    </owl:DatatypeProperty>
    


    <!-- http://www.semanticweb.org/ontologies/2022/2/CDS_V0.6.owl#Outbound_model_version -->


    <owl:DatatypeProperty rdf:about="http://www.semanticweb.org/ontologies/2022/2/CDS_V0.6.owl#Outbound_model_version">
        <rdfs:domain rdf:resource="http://www.semanticweb.org/ontologies/2022/2/CDS_V0.6.owl#Ecosystem_Component"/>
        <rdfs:range rdf:resource="http://www.w3.org/2001/XMLSchema#string"/>
        <rdfs:comment xml:lang="en">Information Model version being produced by the Ecosystem Component</rdfs:comment>
    </owl:DatatypeProperty>
    


    <!-- http://www.semanticweb.org/ontologies/2022/2/CDS_V0.6.owl#Outbound_topic -->


    <owl:DatatypeProperty rdf:about="http://www.semanticweb.org/ontologies/2022/2/CDS_V0.6.owl#Outbound_topic">
        <rdfs:domain rdf:resource="http://www.semanticweb.org/ontologies/2022/2/CDS_V0.6.owl#Endpoint"/>
        <rdfs:range rdf:resource="http://www.w3.org/2001/XMLSchema#string"/>
        <rdfs:comment xml:lang="en">Relative path used for outbound communication via this endpoint, i.e. output messages and faults only.</rdfs:comment>
    </owl:DatatypeProperty>
    


    <!-- http://www.semanticweb.org/ontologies/2022/2/CDS_V0.6.owl#Participant_Certification_Level -->


    <owl:DatatypeProperty rdf:about="http://www.semanticweb.org/ontologies/2022/2/CDS_V0.6.owl#Participant_Certification_Level">
        <rdfs:domain rdf:resource="http://www.semanticweb.org/ontologies/2022/2/CDS_V0.6.owl#Participant_Certification"/>
        <rdfs:range rdf:resource="http://www.w3.org/2001/XMLSchema#string"/>
        <rdfs:comment xml:lang="en">Level of a Participant Certification</rdfs:comment>
    </owl:DatatypeProperty>
    


    <!-- http://www.semanticweb.org/ontologies/2022/2/CDS_V0.6.owl#Participant_Provenance -->


    <owl:DatatypeProperty rdf:about="http://www.semanticweb.org/ontologies/2022/2/CDS_V0.6.owl#Participant_Provenance">
        <rdfs:domain rdf:resource="http://www.semanticweb.org/ontologies/2022/2/CDS_V0.6.owl#Broker"/>
        <rdfs:domain rdf:resource="http://www.semanticweb.org/ontologies/2022/2/CDS_V0.6.owl#Resource"/>
        <rdfs:range rdf:resource="http://www.w3.org/2001/XMLSchema#string"/>
        <rdfs:comment xml:lang="en">Participants that are responsible of trace the Content Provenance</rdfs:comment>
    </owl:DatatypeProperty>
    


    <!-- http://www.semanticweb.org/ontologies/2022/2/CDS_V0.6.owl#Payment_plan -->


    <owl:DatatypeProperty rdf:about="http://www.semanticweb.org/ontologies/2022/2/CDS_V0.6.owl#Payment_plan">
        <rdfs:domain rdf:resource="http://www.semanticweb.org/ontologies/2022/2/CDS_V0.6.owl#Wallet"/>
        <rdfs:range rdf:resource="http://www.w3.org/2001/XMLSchema#string"/>
        <rdfs:comment xml:lang="en">Payment plan associated to a Participant</rdfs:comment>
    </owl:DatatypeProperty>
    


    <!-- http://www.semanticweb.org/ontologies/2022/2/CDS_V0.6.owl#PostalAddress -->


    <owl:DatatypeProperty rdf:about="http://www.semanticweb.org/ontologies/2022/2/CDS_V0.6.owl#PostalAddress">
        <rdfs:domain rdf:resource="http://www.semanticweb.org/ontologies/2022/2/CDS_V0.6.owl#Person"/>
        <rdfs:range rdf:resource="http://www.w3.org/2001/XMLSchema#string"/>
        <rdfs:comment xml:lang="en">Physical address of the item</rdfs:comment>
    </owl:DatatypeProperty>
    


    <!-- http://www.semanticweb.org/ontologies/2022/2/CDS_V0.6.owl#Pricing_strategy -->


    <owl:DatatypeProperty rdf:about="http://www.semanticweb.org/ontologies/2022/2/CDS_V0.6.owl#Pricing_strategy">
        <rdfs:domain rdf:resource="http://www.semanticweb.org/ontologies/2022/2/CDS_V0.6.owl#Resource"/>
        <rdfs:range rdf:resource="http://www.w3.org/2001/XMLSchema#string"/>
        <dc:contributor xml:lang="en">The Free strategy does not charge the usage of resources. 
The Freemium strategy exposes a limited parts (or capabilities) of the resource at no cost, while additional parts are charged Pay-per-Use, or based on a Flat Rate. 
The Pay-per-Use strategy relies on a particular metrics (volume, access count, download) to define a charged instance of usage.
The Flat Rate strategy charges usage per quantitative slot (time, volume, credit), optionally associated with a tiered cost model according to the configuration of the retrieved resource.</dc:contributor>
    </owl:DatatypeProperty>
    


    <!-- http://www.semanticweb.org/ontologies/2022/2/CDS_V0.6.owl#PublicationDate -->


    <owl:DatatypeProperty rdf:about="http://www.semanticweb.org/ontologies/2022/2/CDS_V0.6.owl#PublicationDate">
        <rdfs:domain rdf:resource="http://www.semanticweb.org/ontologies/2022/2/CDS_V0.6.owl#Data_Asset"/>
        <rdfs:range rdf:resource="http://www.w3.org/2001/XMLSchema#string"/>
        <rdfs:comment xml:lang="en">Date of formal issuance (e.g., publication) of the data asset.</rdfs:comment>
    </owl:DatatypeProperty>
    


    <!-- http://www.semanticweb.org/ontologies/2022/2/CDS_V0.6.owl#Recommended_Access_Interface -->


    <owl:DatatypeProperty rdf:about="http://www.semanticweb.org/ontologies/2022/2/CDS_V0.6.owl#Recommended_Access_Interface">
        <rdfs:domain rdf:resource="http://www.semanticweb.org/ontologies/2022/2/CDS_V0.6.owl#Transaction_Data"/>
        <rdfs:range rdf:resource="http://www.w3.org/2001/XMLSchema#string"/>
        <rdfs:comment xml:lang="en">Indication (ID) on the recommended access interface</rdfs:comment>
    </owl:DatatypeProperty>
    


    <!-- http://www.semanticweb.org/ontologies/2022/2/CDS_V0.6.owl#Resource_Identifier -->


    <owl:DatatypeProperty rdf:about="http://www.semanticweb.org/ontologies/2022/2/CDS_V0.6.owl#Resource_Identifier">
        <rdfs:domain rdf:resource="http://www.semanticweb.org/ontologies/2022/2/CDS_V0.6.owl#Resource"/>
        <rdfs:range rdf:resource="http://www.w3.org/2001/XMLSchema#string"/>
        <rdfs:comment xml:lang="en">A unique identifier of the item.</rdfs:comment>
    </owl:DatatypeProperty>
    


    <!-- http://www.semanticweb.org/ontologies/2022/2/CDS_V0.6.owl#Resource_Name -->


    <owl:DatatypeProperty rdf:about="http://www.semanticweb.org/ontologies/2022/2/CDS_V0.6.owl#Resource_Name">
        <rdfs:domain rdf:resource="http://www.semanticweb.org/ontologies/2022/2/CDS_V0.6.owl#Resource"/>
        <rdfs:range rdf:resource="http://www.w3.org/2001/XMLSchema#string"/>
        <rdfs:comment xml:lang="en">A name given to the item.</rdfs:comment>
    </owl:DatatypeProperty>
    


    <!-- http://www.semanticweb.org/ontologies/2022/2/CDS_V0.6.owl#Rights -->


    <owl:DatatypeProperty rdf:about="http://www.semanticweb.org/ontologies/2022/2/CDS_V0.6.owl#Rights">
        <rdfs:domain rdf:resource="http://www.semanticweb.org/ontologies/2022/2/CDS_V0.6.owl#Resource"/>
        <rdfs:range rdf:resource="http://www.w3.org/2001/XMLSchema#string"/>
        <rdfs:comment xml:lang="en">A statement that concerns all rights not addressed with license or accessRights, such as copyright statements.</rdfs:comment>
    </owl:DatatypeProperty>
    


    <!-- http://www.semanticweb.org/ontologies/2022/2/CDS_V0.6.owl#Role -->


    <owl:DatatypeProperty rdf:about="http://www.semanticweb.org/ontologies/2022/2/CDS_V0.6.owl#Role">
        <rdfs:domain rdf:resource="http://www.semanticweb.org/ontologies/2022/2/CDS_V0.6.owl#Participant"/>
        <rdfs:comment xml:lang="en">Service Provider,
Service Consumer,
Data Owner,
Data Provider,
Federator,
Federation user</rdfs:comment>
    </owl:DatatypeProperty>
    


    <!-- http://www.semanticweb.org/ontologies/2022/2/CDS_V0.6.owl#Service_Catalogue_Homepage -->


    <owl:DatatypeProperty rdf:about="http://www.semanticweb.org/ontologies/2022/2/CDS_V0.6.owl#Service_Catalogue_Homepage">
        <rdfs:domain rdf:resource="http://www.semanticweb.org/ontologies/2022/2/CDS_V0.6.owl#Service_Catalogue"/>
        <rdfs:range rdf:resource="http://www.w3.org/2001/XMLSchema#anyURI"/>
        <rdfs:comment xml:lang="en">A homepage of the Service Catalogue.</rdfs:comment>
    </owl:DatatypeProperty>
    


    <!-- http://www.semanticweb.org/ontologies/2022/2/CDS_V0.6.owl#Service_Catalogue_curator -->


    <owl:DatatypeProperty rdf:about="http://www.semanticweb.org/ontologies/2022/2/CDS_V0.6.owl#Service_Catalogue_curator">
        <rdfs:domain rdf:resource="http://www.semanticweb.org/ontologies/2022/2/CDS_V0.6.owl#Service_Catalogue"/>
        <rdfs:range rdf:resource="http://www.w3.org/2001/XMLSchema#string"/>
        <rdfs:comment xml:lang="en">Participant responsible for technical maintenance of the Ecosystem Component.</rdfs:comment>
    </owl:DatatypeProperty>
    


    <!-- http://www.semanticweb.org/ontologies/2022/2/CDS_V0.6.owl#Service_Catalogue_maintainer -->


    <owl:DatatypeProperty rdf:about="http://www.semanticweb.org/ontologies/2022/2/CDS_V0.6.owl#Service_Catalogue_maintainer">
        <rdfs:domain rdf:resource="http://www.semanticweb.org/ontologies/2022/2/CDS_V0.6.owl#Service_Catalogue"/>
        <rdfs:range rdf:resource="http://www.w3.org/2001/XMLSchema#string"/>
        <rdfs:comment xml:lang="en">Descriptive information on the Participant responsible for the correctness of the content offered by the Ecosystem Component.</rdfs:comment>
    </owl:DatatypeProperty>
    


    <!-- http://www.semanticweb.org/ontologies/2022/2/CDS_V0.6.owl#Service_Name -->


    <owl:DatatypeProperty rdf:about="http://www.semanticweb.org/ontologies/2022/2/CDS_V0.6.owl#Service_Name">
        <rdfs:domain rdf:resource="http://www.semanticweb.org/ontologies/2022/2/CDS_V0.6.owl#Data_Service"/>
        <rdfs:range rdf:resource="http://www.w3.org/2001/XMLSchema#string"/>
        <rdfs:comment xml:lang="en">Name of the Service.
</rdfs:comment>
    </owl:DatatypeProperty>
    


    <!-- http://www.semanticweb.org/ontologies/2022/2/CDS_V0.6.owl#SiteAddress -->


    <owl:DatatypeProperty rdf:about="http://www.semanticweb.org/ontologies/2022/2/CDS_V0.6.owl#SiteAddress">
        <rdfs:domain rdf:resource="http://www.semanticweb.org/ontologies/2022/2/CDS_V0.6.owl#Participant"/>
        <rdfs:range rdf:resource="http://www.w3.org/2001/XMLSchema#string"/>
        <rdfs:comment xml:lang="en">Address of an office or other premise at which the organization is located.
It is particularly important in cases in which specific rules (e.g., national law) apply, affecting, for example, the data usage control policy.</rdfs:comment>
    </owl:DatatypeProperty>
    


    <!-- http://www.semanticweb.org/ontologies/2022/2/CDS_V0.6.owl#Surname -->


    <owl:DatatypeProperty rdf:about="http://www.semanticweb.org/ontologies/2022/2/CDS_V0.6.owl#Surname">
        <rdfs:domain rdf:resource="http://www.semanticweb.org/ontologies/2022/2/CDS_V0.6.owl#Person"/>
        <rdfs:range rdf:resource="http://www.w3.org/2001/XMLSchema#string"/>
        <rdfs:comment xml:lang="en">Surname of the Person</rdfs:comment>
    </owl:DatatypeProperty>
    


    <!-- http://www.semanticweb.org/ontologies/2022/2/CDS_V0.6.owl#Volume_transf -->


    <owl:DatatypeProperty rdf:about="http://www.semanticweb.org/ontologies/2022/2/CDS_V0.6.owl#Volume_transf">
        <rdfs:domain rdf:resource="http://www.semanticweb.org/ontologies/2022/2/CDS_V0.6.owl#Transaction_Data"/>
        <rdfs:range rdf:resource="http://www.w3.org/2001/XMLSchema#float"/>
        <rdfs:comment xml:lang="en">Indication of the data transfer volumes, as percentage with respect to the total user level data volume</rdfs:comment>
    </owl:DatatypeProperty>
    


    <!-- http://www.semanticweb.org/ontologies/2022/2/CDS_V0.6.owl#Wallet_Homepage -->


    <owl:DatatypeProperty rdf:about="http://www.semanticweb.org/ontologies/2022/2/CDS_V0.6.owl#Wallet_Homepage">
        <rdfs:domain rdf:resource="http://www.semanticweb.org/ontologies/2022/2/CDS_V0.6.owl#Wallet"/>
        <rdfs:range rdf:resource="http://www.w3.org/2001/XMLSchema#anyURI"/>
        <rdfs:comment xml:lang="en">A homepage of the Wallet service.</rdfs:comment>
    </owl:DatatypeProperty>
    


    <!-- http://www.semanticweb.org/ontologies/2022/2/CDS_V0.6.owl#Wallet_Identifier -->


    <owl:DatatypeProperty rdf:about="http://www.semanticweb.org/ontologies/2022/2/CDS_V0.6.owl#Wallet_Identifier">
        <rdfs:domain rdf:resource="http://www.semanticweb.org/ontologies/2022/2/CDS_V0.6.owl#Wallet"/>
        <rdfs:range rdf:resource="http://www.w3.org/2001/XMLSchema#string"/>
        <rdfs:comment xml:lang="en">Unique identifier of a Participant’s wallet</rdfs:comment>
    </owl:DatatypeProperty>
    


    <!-- http://www.semanticweb.org/ontologies/2022/2/CDS_V0.6.owl#Wallet_curator -->


    <owl:DatatypeProperty rdf:about="http://www.semanticweb.org/ontologies/2022/2/CDS_V0.6.owl#Wallet_curator">
        <rdfs:domain rdf:resource="http://www.semanticweb.org/ontologies/2022/2/CDS_V0.6.owl#Wallet"/>
        <rdfs:range rdf:resource="http://www.w3.org/2001/XMLSchema#string"/>
        <rdfs:comment xml:lang="en">Participant responsible for technical maintenance of the Ecosystem Component.</rdfs:comment>
    </owl:DatatypeProperty>
    


    <!-- http://www.semanticweb.org/ontologies/2022/2/CDS_V0.6.owl#Wallet_maintainer -->


    <owl:DatatypeProperty rdf:about="http://www.semanticweb.org/ontologies/2022/2/CDS_V0.6.owl#Wallet_maintainer">
        <rdfs:domain rdf:resource="http://www.semanticweb.org/ontologies/2022/2/CDS_V0.6.owl#Wallet"/>
        <rdfs:range rdf:resource="http://www.w3.org/2001/XMLSchema#string"/>
        <rdfs:comment xml:lang="en">Descriptive information on the Participant responsible for the correctness of the content offered by the Ecosystem Component.</rdfs:comment>
    </owl:DatatypeProperty>
    


    <!-- http://www.semanticweb.org/ontologies/2022/2/CDS_V0.6.owl#action -->


    <owl:DatatypeProperty rdf:about="http://www.semanticweb.org/ontologies/2022/2/CDS_V0.6.owl#action">
        <rdfs:domain rdf:resource="http://www.semanticweb.org/ontologies/2022/2/CDS_V0.6.owl#Contract"/>
        <rdfs:domain rdf:resource="http://www.semanticweb.org/ontologies/2022/2/CDS_V0.6.owl#Rule"/>
        <rdfs:domain rdf:resource="http://www.semanticweb.org/ontologies/2022/2/CDS_V0.6.owl#Transaction_Data"/>
        <rdfs:range rdf:resource="http://www.w3.org/2001/XMLSchema#string"/>
        <rdfs:comment xml:lang="en">Descriptive information on the action</rdfs:comment>
    </owl:DatatypeProperty>
    


    <!-- http://www.semanticweb.org/ontologies/2022/2/CDS_V0.6.owl#actionPerformer -->


    <owl:DatatypeProperty rdf:about="http://www.semanticweb.org/ontologies/2022/2/CDS_V0.6.owl#actionPerformer">
        <rdfs:domain rdf:resource="http://www.semanticweb.org/ontologies/2022/2/CDS_V0.6.owl#Action"/>
        <rdfs:range rdf:resource="http://www.w3.org/2001/XMLSchema#string"/>
        <rdfs:comment xml:lang="en">Participant performer of the Action</rdfs:comment>
    </owl:DatatypeProperty>
    


    <!-- http://www.semanticweb.org/ontologies/2022/2/CDS_V0.6.owl#actionStatus -->


    <owl:DatatypeProperty rdf:about="http://www.semanticweb.org/ontologies/2022/2/CDS_V0.6.owl#actionStatus">
        <rdfs:domain rdf:resource="http://www.semanticweb.org/ontologies/2022/2/CDS_V0.6.owl#Action"/>
        <rdfs:range rdf:resource="http://www.w3.org/2001/XMLSchema#string"/>
        <rdfs:comment xml:lang="en">Indicates the current disposition of the Action.
In-progress, completed, failed, potential.</rdfs:comment>
    </owl:DatatypeProperty>
    


    <!-- http://www.semanticweb.org/ontologies/2022/2/CDS_V0.6.owl#assignee -->


    <owl:DatatypeProperty rdf:about="http://www.semanticweb.org/ontologies/2022/2/CDS_V0.6.owl#assignee">
        <rdfs:domain rdf:resource="http://www.semanticweb.org/ontologies/2022/2/CDS_V0.6.owl#Contract_agreement"/>
        <rdfs:domain rdf:resource="http://www.semanticweb.org/ontologies/2022/2/CDS_V0.6.owl#Contract_request"/>
        <rdfs:domain rdf:resource="http://www.semanticweb.org/ontologies/2022/2/CDS_V0.6.owl#Rule"/>
        <rdfs:range rdf:resource="http://www.w3.org/2001/XMLSchema#string"/>
        <rdfs:comment xml:lang="en">Descriptive information on the assignee Participant.</rdfs:comment>
    </owl:DatatypeProperty>
    


    <!-- http://www.semanticweb.org/ontologies/2022/2/CDS_V0.6.owl#assigner -->


    <owl:DatatypeProperty rdf:about="http://www.semanticweb.org/ontologies/2022/2/CDS_V0.6.owl#assigner">
        <rdfs:domain rdf:resource="http://www.semanticweb.org/ontologies/2022/2/CDS_V0.6.owl#Contract_agreement"/>
        <rdfs:domain rdf:resource="http://www.semanticweb.org/ontologies/2022/2/CDS_V0.6.owl#Contract_offer"/>
        <rdfs:domain rdf:resource="http://www.semanticweb.org/ontologies/2022/2/CDS_V0.6.owl#Contract_request"/>
        <rdfs:domain rdf:resource="http://www.semanticweb.org/ontologies/2022/2/CDS_V0.6.owl#Rule"/>
        <rdfs:range rdf:resource="http://www.w3.org/2001/XMLSchema#string"/>
        <rdfs:comment xml:lang="en">Descriptive information on the assigner Participant.</rdfs:comment>
    </owl:DatatypeProperty>
    


    <!-- http://www.semanticweb.org/ontologies/2022/2/CDS_V0.6.owl#authInfo -->


    <owl:DatatypeProperty rdf:about="http://www.semanticweb.org/ontologies/2022/2/CDS_V0.6.owl#authInfo">
        <rdfs:domain rdf:resource="http://www.semanticweb.org/ontologies/2022/2/CDS_V0.6.owl#Connector"/>
        <rdfs:range rdf:resource="http://www.w3.org/2001/XMLSchema#string"/>
        <rdfs:comment xml:lang="en">Information of the authentication server used by the Connector</rdfs:comment>
    </owl:DatatypeProperty>
    


    <!-- http://www.semanticweb.org/ontologies/2022/2/CDS_V0.6.owl#certification_type -->


    <owl:DatatypeProperty rdf:about="http://www.semanticweb.org/ontologies/2022/2/CDS_V0.6.owl#certification_type">
        <rdfs:domain rdf:resource="http://www.semanticweb.org/ontologies/2022/2/CDS_V0.6.owl#Certification"/>
        <rdfs:comment xml:lang="en">Type of the certification issued (e.g. X509)</rdfs:comment>
    </owl:DatatypeProperty>
    


    <!-- http://www.semanticweb.org/ontologies/2022/2/CDS_V0.6.owl#constraint -->


    <owl:DatatypeProperty rdf:about="http://www.semanticweb.org/ontologies/2022/2/CDS_V0.6.owl#constraint">
        <rdfs:domain rdf:resource="http://www.semanticweb.org/ontologies/2022/2/CDS_V0.6.owl#Rule"/>
        <rdfs:range rdf:resource="http://www.w3.org/2001/XMLSchema#string"/>
        <rdfs:comment xml:lang="en">Descriptive information on the Constraint applied to the Rule.</rdfs:comment>
    </owl:DatatypeProperty>
    


    <!-- http://www.semanticweb.org/ontologies/2022/2/CDS_V0.6.owl#corporateEmailAddress -->


    <owl:DatatypeProperty rdf:about="http://www.semanticweb.org/ontologies/2022/2/CDS_V0.6.owl#corporateEmailAddress">
        <rdfs:domain rdf:resource="http://www.semanticweb.org/ontologies/2022/2/CDS_V0.6.owl#Participant"/>
        <rdfs:range rdf:resource="http://www.w3.org/2001/XMLSchema#string"/>
        <rdfs:comment xml:lang="en">Email Address of the Participant</rdfs:comment>
    </owl:DatatypeProperty>
    


    <!-- http://www.semanticweb.org/ontologies/2022/2/CDS_V0.6.owl#corporateHomepage -->


    <owl:DatatypeProperty rdf:about="http://www.semanticweb.org/ontologies/2022/2/CDS_V0.6.owl#corporateHomepage">
        <rdfs:domain rdf:resource="http://www.semanticweb.org/ontologies/2022/2/CDS_V0.6.owl#Participant"/>
        <rdfs:range rdf:resource="http://www.w3.org/2001/XMLSchema#anyURI"/>
        <rdfs:comment xml:lang="en">Homepage of the Participant</rdfs:comment>
    </owl:DatatypeProperty>
    


    <!-- http://www.semanticweb.org/ontologies/2022/2/CDS_V0.6.owl#datatype -->


    <owl:DatatypeProperty rdf:about="http://www.semanticweb.org/ontologies/2022/2/CDS_V0.6.owl#datatype">
        <rdfs:domain rdf:resource="http://www.semanticweb.org/ontologies/2022/2/CDS_V0.6.owl#Constraint"/>
        <rdfs:comment xml:lang="en">The datatype of the value of the rightOperand or rightOperandReference of a Constraint.</rdfs:comment>
    </owl:DatatypeProperty>
    


    <!-- http://www.semanticweb.org/ontologies/2022/2/CDS_V0.6.owl#description -->


    <owl:DatatypeProperty rdf:about="http://www.semanticweb.org/ontologies/2022/2/CDS_V0.6.owl#description">
        <rdfs:domain rdf:resource="http://www.semanticweb.org/ontologies/2022/2/CDS_V0.6.owl#Resource"/>
        <rdfs:range rdf:resource="http://www.w3.org/2001/XMLSchema#string"/>
        <rdfs:comment xml:lang="en">A free-text account of the item</rdfs:comment>
    </owl:DatatypeProperty>
    


    <!-- http://www.semanticweb.org/ontologies/2022/2/CDS_V0.6.owl#endTime -->


    <owl:DatatypeProperty rdf:about="http://www.semanticweb.org/ontologies/2022/2/CDS_V0.6.owl#endTime">
        <rdfs:domain rdf:resource="http://www.semanticweb.org/ontologies/2022/2/CDS_V0.6.owl#Action"/>
        <rdfs:range rdf:resource="http://www.w3.org/2001/XMLSchema#dateTime"/>
        <rdfs:comment xml:lang="en">The end time of an action.</rdfs:comment>
    </owl:DatatypeProperty>
    


    <!-- http://www.semanticweb.org/ontologies/2022/2/CDS_V0.6.owl#error -->


    <owl:DatatypeProperty rdf:about="http://www.semanticweb.org/ontologies/2022/2/CDS_V0.6.owl#error">
        <rdfs:domain rdf:resource="http://www.semanticweb.org/ontologies/2022/2/CDS_V0.6.owl#Action"/>
        <rdfs:range rdf:resource="http://www.w3.org/2001/XMLSchema#string"/>
        <rdfs:comment xml:lang="en">Descriptive information on the cause of the failure (optional, for failed actions)</rdfs:comment>
    </owl:DatatypeProperty>
    


    <!-- http://www.semanticweb.org/ontologies/2022/2/CDS_V0.6.owl#format -->


    <owl:DatatypeProperty rdf:about="http://www.semanticweb.org/ontologies/2022/2/CDS_V0.6.owl#format">
        <rdfs:domain rdf:resource="http://www.semanticweb.org/ontologies/2022/2/CDS_V0.6.owl#Resource"/>
        <rdfs:range rdf:resource="http://www.w3.org/2001/XMLSchema#string"/>
        <rdfs:comment xml:lang="en">Resource format.</rdfs:comment>
    </owl:DatatypeProperty>
    


    <!-- http://www.semanticweb.org/ontologies/2022/2/CDS_V0.6.owl#indexed_metadatum -->


    <owl:DatatypeProperty rdf:about="http://www.semanticweb.org/ontologies/2022/2/CDS_V0.6.owl#indexed_metadatum">
        <rdfs:domain rdf:resource="http://www.semanticweb.org/ontologies/2022/2/CDS_V0.6.owl#Broker"/>
        <rdfs:comment xml:lang="en">Metadatum indexed in the Broker</rdfs:comment>
    </owl:DatatypeProperty>
    


    <!-- http://www.semanticweb.org/ontologies/2022/2/CDS_V0.6.owl#infoDataService -->


    <owl:DatatypeProperty rdf:about="http://www.semanticweb.org/ontologies/2022/2/CDS_V0.6.owl#infoDataService">
        <rdfs:domain rdf:resource="http://www.semanticweb.org/ontologies/2022/2/CDS_V0.6.owl#Transaction_Data"/>
        <rdfs:range rdf:resource="http://www.w3.org/2001/XMLSchema#string"/>
        <rdfs:comment xml:lang="en">Descriptive information on the data service that allowed the action</rdfs:comment>
    </owl:DatatypeProperty>
    


    <!-- http://www.semanticweb.org/ontologies/2022/2/CDS_V0.6.owl#leftOperand -->


    <owl:DatatypeProperty rdf:about="http://www.semanticweb.org/ontologies/2022/2/CDS_V0.6.owl#leftOperand">
        <rdfs:domain rdf:resource="http://www.semanticweb.org/ontologies/2022/2/CDS_V0.6.owl#Constraint"/>
        <rdfs:range rdf:resource="http://www.w3.org/2001/XMLSchema#string"/>
        <rdfs:comment xml:lang="en">The left operand in a constraint expression. The leftOperand instances must clearly be defined to indicate the semantics of the Constraint, and may declare how the value for comparison has to be retrieved or generated.
Example: Absolute geo-spatial position, count, current event, delay, elapsed time, endpoint, execution system, path to attribute, payAmount, payment, policy evaluation time, purpose, quantity, recurrence rate, security level, state, user.</rdfs:comment>
    </owl:DatatypeProperty>
    


    <!-- http://www.semanticweb.org/ontologies/2022/2/CDS_V0.6.owl#operator -->


    <owl:DatatypeProperty rdf:about="http://www.semanticweb.org/ontologies/2022/2/CDS_V0.6.owl#operator">
        <rdfs:domain rdf:resource="http://www.semanticweb.org/ontologies/2022/2/CDS_V0.6.owl#Constraint"/>
        <rdfs:range rdf:resource="http://www.w3.org/2001/XMLSchema#string"/>
        <rdfs:comment xml:lang="en">The operator instances identify the relational operation between the left and right operands.
Example: after, before, contains, covered by, covers, defines as, disjoint, during, equals, finished by, finishes, greater than, greater than or equals, has Member, has same duration, has site, has state, inside, inside network, interval equals, is same as, less than or equals, longer, longer or equals, matches, meet, meets, memberOf, met by, not equals, overlap, overlapped by, overlaps, shorter, shorter or equals, started by, starts, string contains, string equals, string is contained in.</rdfs:comment>
    </owl:DatatypeProperty>
    


    <!-- http://www.semanticweb.org/ontologies/2022/2/CDS_V0.6.owl#organization -->


    <owl:DatatypeProperty rdf:about="http://www.semanticweb.org/ontologies/2022/2/CDS_V0.6.owl#organization">
        <rdfs:domain rdf:resource="http://www.semanticweb.org/ontologies/2022/2/CDS_V0.6.owl#Person"/>
        <rdfs:range rdf:resource="http://www.w3.org/2001/XMLSchema#string"/>
        <rdfs:comment xml:lang="en">An organization that this person is affiliated with.</rdfs:comment>
    </owl:DatatypeProperty>
    


    <!-- http://www.semanticweb.org/ontologies/2022/2/CDS_V0.6.owl#path -->


    <owl:DatatypeProperty rdf:about="http://www.semanticweb.org/ontologies/2022/2/CDS_V0.6.owl#path">
        <rdfs:domain rdf:resource="http://www.semanticweb.org/ontologies/2022/2/CDS_V0.6.owl#Endpoint"/>
        <rdfs:range rdf:resource="http://www.w3.org/2001/XMLSchema#string"/>
        <rdfs:comment xml:lang="en">Relative path, topic or queue at which the content is published by the related host.</rdfs:comment>
    </owl:DatatypeProperty>
    


    <!-- http://www.semanticweb.org/ontologies/2022/2/CDS_V0.6.owl#phoneNumber -->


    <owl:DatatypeProperty rdf:about="http://www.semanticweb.org/ontologies/2022/2/CDS_V0.6.owl#phoneNumber">
        <rdfs:domain rdf:resource="http://www.semanticweb.org/ontologies/2022/2/CDS_V0.6.owl#Person"/>
        <rdfs:range rdf:resource="http://www.w3.org/2001/XMLSchema#string"/>
        <rdfs:comment xml:lang="en">Phone number of the Person</rdfs:comment>
    </owl:DatatypeProperty>
    


    <!-- http://www.semanticweb.org/ontologies/2022/2/CDS_V0.6.owl#rightOperand -->


    <owl:DatatypeProperty rdf:about="http://www.semanticweb.org/ontologies/2022/2/CDS_V0.6.owl#rightOperand">
        <rdfs:domain rdf:resource="http://www.semanticweb.org/ontologies/2022/2/CDS_V0.6.owl#Constraint"/>
        <rdfs:range rdf:resource="http://www.w3.org/2000/01/rdf-schema#Literal"/>
        <rdfs:comment xml:lang="en">The rightOperand is the value of the Constraint that is to be compared to the leftOperand.</rdfs:comment>
    </owl:DatatypeProperty>
    


    <!-- http://www.semanticweb.org/ontologies/2022/2/CDS_V0.6.owl#rightOperandReference -->


    <owl:DatatypeProperty rdf:about="http://www.semanticweb.org/ontologies/2022/2/CDS_V0.6.owl#rightOperandReference">
        <rdfs:domain rdf:resource="http://www.semanticweb.org/ontologies/2022/2/CDS_V0.6.owl#Constraint"/>
        <rdfs:range rdf:resource="http://www.w3.org/2000/01/rdf-schema#Literal"/>
        <rdfs:comment xml:lang="en">A reference to a web resource providing the value for the right operand of a Constraint.</rdfs:comment>
    </owl:DatatypeProperty>
    


    <!-- http://www.semanticweb.org/ontologies/2022/2/CDS_V0.6.owl#rule -->


    <owl:DatatypeProperty rdf:about="http://www.semanticweb.org/ontologies/2022/2/CDS_V0.6.owl#rule">
        <rdfs:domain rdf:resource="http://www.semanticweb.org/ontologies/2022/2/CDS_V0.6.owl#Contract"/>
        <rdfs:range rdf:resource="http://www.w3.org/2001/XMLSchema#string"/>
        <rdfs:comment xml:lang="en">Descriptive information on Rule represented by the Contract Offer (permission, prohibition, obligation)</rdfs:comment>
    </owl:DatatypeProperty>
    


    <!-- http://www.semanticweb.org/ontologies/2022/2/CDS_V0.6.owl#startTime -->


    <owl:DatatypeProperty rdf:about="http://www.semanticweb.org/ontologies/2022/2/CDS_V0.6.owl#startTime">
        <rdfs:domain rdf:resource="http://www.semanticweb.org/ontologies/2022/2/CDS_V0.6.owl#Action"/>
        <rdfs:range rdf:resource="http://www.w3.org/2001/XMLSchema#dateTime"/>
        <rdfs:comment xml:lang="en">The start time of an action.</rdfs:comment>
    </owl:DatatypeProperty>
    


    <!-- http://www.semanticweb.org/ontologies/2022/2/CDS_V0.6.owl#status -->


    <owl:DatatypeProperty rdf:about="http://www.semanticweb.org/ontologies/2022/2/CDS_V0.6.owl#status">
        <rdfs:domain rdf:resource="http://www.semanticweb.org/ontologies/2022/2/CDS_V0.6.owl#Constraint"/>
        <rdfs:comment xml:lang="en">The status provides a value generated from the leftOperand action that must be used in the comparison expression</rdfs:comment>
    </owl:DatatypeProperty>
    


    <!-- http://www.semanticweb.org/ontologies/2022/2/CDS_V0.6.owl#target -->


    <owl:DatatypeProperty rdf:about="http://www.semanticweb.org/ontologies/2022/2/CDS_V0.6.owl#target">
        <rdfs:domain rdf:resource="http://www.semanticweb.org/ontologies/2022/2/CDS_V0.6.owl#Contract"/>
        <rdfs:domain rdf:resource="http://www.semanticweb.org/ontologies/2022/2/CDS_V0.6.owl#Rule"/>
        <rdfs:range rdf:resource="http://www.w3.org/2001/XMLSchema#string"/>
        <rdfs:comment xml:lang="en">Descriptive information on resource subject of the Rule</rdfs:comment>
    </owl:DatatypeProperty>
    


    <!-- http://www.semanticweb.org/ontologies/2022/2/CDS_V0.6.owl#target_EntryPoint -->


    <owl:DatatypeProperty rdf:about="http://www.semanticweb.org/ontologies/2022/2/CDS_V0.6.owl#target_EntryPoint">
        <rdfs:domain rdf:resource="http://www.semanticweb.org/ontologies/2022/2/CDS_V0.6.owl#Action"/>
        <rdfs:range rdf:resource="http://www.w3.org/2001/XMLSchema#anyURI"/>
        <rdfs:comment xml:lang="en">An entrypoint used to execute the action.</rdfs:comment>
    </owl:DatatypeProperty>
    


    <!-- http://www.semanticweb.org/ontologies/2022/2/CDS_V0.6.owl#taxonomy -->


    <owl:DatatypeProperty rdf:about="http://www.semanticweb.org/ontologies/2022/2/CDS_V0.6.owl#taxonomy">
        <rdfs:domain rdf:resource="http://www.semanticweb.org/ontologies/2022/2/CDS_V0.6.owl#Data_App"/>
        <rdfs:range rdf:resource="http://www.w3.org/2001/XMLSchema#string"/>
        <rdfs:comment xml:lang="en">Data Providing App,
and/or
Data Processing App,
and/or
Data Consuming App.</rdfs:comment>
    </owl:DatatypeProperty>
    


    <!-- http://www.semanticweb.org/ontologies/2022/2/CDS_V0.6.owl#transactionUser -->


    <owl:DatatypeProperty rdf:about="http://www.semanticweb.org/ontologies/2022/2/CDS_V0.6.owl#transactionUser">
        <rdfs:domain rdf:resource="http://www.semanticweb.org/ontologies/2022/2/CDS_V0.6.owl#Transaction_Data"/>
        <rdfs:range rdf:resource="http://www.w3.org/2001/XMLSchema#string"/>
        <rdfs:comment xml:lang="en">Descriptive information on the Participant responsible of the transaction</rdfs:comment>
    </owl:DatatypeProperty>
    


    <!-- http://www.semanticweb.org/ontologies/2022/2/CDS_V0.6.owl#unit -->


    <owl:DatatypeProperty rdf:about="http://www.semanticweb.org/ontologies/2022/2/CDS_V0.6.owl#unit">
        <rdfs:domain rdf:resource="http://www.semanticweb.org/ontologies/2022/2/CDS_V0.6.owl#Constraint"/>
        <rdfs:comment xml:lang="en">unit indicates the unit value of the rightOperand/Reference.</rdfs:comment>
    </owl:DatatypeProperty>
    


    <!-- http://www.semanticweb.org/ontologies/2022/2/CDS_V0.6.owl#version -->


    <owl:DatatypeProperty rdf:about="http://www.semanticweb.org/ontologies/2022/2/CDS_V0.6.owl#version">
        <rdfs:domain rdf:resource="http://www.semanticweb.org/ontologies/2022/2/CDS_V0.6.owl#Managed_Entity"/>
        <rdfs:range rdf:resource="http://www.w3.org/2001/XMLSchema#string"/>
        <rdfs:comment xml:lang="en">Version identified of the Managed Entity.
</rdfs:comment>
    </owl:DatatypeProperty>
    


    <!-- http://www.semanticweb.org/ontologies/2022/2/CDS_V0.6.owl#walletAmount -->


    <owl:DatatypeProperty rdf:about="http://www.semanticweb.org/ontologies/2022/2/CDS_V0.6.owl#walletAmount">
        <rdfs:domain rdf:resource="http://www.semanticweb.org/ontologies/2022/2/CDS_V0.6.owl#Wallet"/>
        <rdfs:range rdf:resource="http://www.w3.org/2001/XMLSchema#float"/>
        <rdfs:comment xml:lang="en">Amount of the wallet, in euros</rdfs:comment>
    </owl:DatatypeProperty>
    


    <!-- http://www.semanticweb.org/ontologies/2022/2/CDS_V0.6.owl#Failure(Tbd)s -->


    <owl:DatatypeProperty rdf:about="http://www.semanticweb.org/ontologies/2022/2/CDS_V0.6.owl#Failure(Tbd)s">
        <rdfs:domain rdf:resource="http://www.semanticweb.org/ontologies/2022/2/CDS_V0.6.owl#Rule"/>
        <rdfs:range rdf:resource="http://www.w3.org/2001/XMLSchema#string"/>
        <rdfs:comment xml:lang="en">violation (or unmet) relationship between Rules.</rdfs:comment>
    </owl:DatatypeProperty>
    


    <!-- 
    ///////////////////////////////////////////////////////////////////////////////////////
    //
    // Classes
    //
    ///////////////////////////////////////////////////////////////////////////////////////
     -->


    


    <!-- http://www.semanticweb.org/ontologies/2022/2/CDS_V0.6.owl#Abstract_Constraint -->


    <owl:Class rdf:about="http://www.semanticweb.org/ontologies/2022/2/CDS_V0.6.owl#Abstract_Constraint">
        <rdfs:comment xml:lang="en">The upper class of Constraints and LogicalConstraints is solely intended as a placeholder at the range of CDS Properties.</rdfs:comment>
    </owl:Class>
    


    <!-- http://www.semanticweb.org/ontologies/2022/2/CDS_V0.6.owl#Action -->


    <owl:Class rdf:about="http://www.semanticweb.org/ontologies/2022/2/CDS_V0.6.owl#Action">
        <rdfs:comment xml:lang="en">An operation that can be exercised on a Resource.</rdfs:comment>
    </owl:Class>
    


    <!-- http://www.semanticweb.org/ontologies/2022/2/CDS_V0.6.owl#Broker -->


    <owl:Class rdf:about="http://www.semanticweb.org/ontologies/2022/2/CDS_V0.6.owl#Broker">
        <rdfs:subClassOf rdf:resource="http://www.semanticweb.org/ontologies/2022/2/CDS_V0.6.owl#Connector"/>
        <rdfs:comment xml:lang="en">Broker holding an index of published data endpoints.
The brokers provide services for real-time data search and discovery, funded on a common and shared information model of data assets.
The Metadata Broker Service Provider is an intermediary that stores and manages information about the data and data sources available in the ecosystem. Its primary task is receiving and providing metadata, via a dedicated and standard interface (e.g., REST). It provides the required metadata for the consumer to connect to a service provider of data assets.</rdfs:comment>
    </owl:Class>
    


    <!-- http://www.semanticweb.org/ontologies/2022/2/CDS_V0.6.owl#Certification -->


    <owl:Class rdf:about="http://www.semanticweb.org/ontologies/2022/2/CDS_V0.6.owl#Certification">
        <rdfs:subClassOf rdf:resource="http://www.semanticweb.org/ontologies/2022/2/CDS_V0.6.owl#Managed_Entity"/>
        <rdfs:comment xml:lang="en">Abstract certification of compliance according to given Certification Scheme.</rdfs:comment>
    </owl:Class>
    


    <!-- http://www.semanticweb.org/ontologies/2022/2/CDS_V0.6.owl#Clearing_House -->


    <owl:Class rdf:about="http://www.semanticweb.org/ontologies/2022/2/CDS_V0.6.owl#Clearing_House">
        <rdfs:subClassOf rdf:resource="http://www.semanticweb.org/ontologies/2022/2/CDS_V0.6.owl#Ecosystem_Component"/>
        <rdfs:comment xml:lang="en">The Clearing House provides clearing and settlement services B2B interactions within the Copernicus Data Space.</rdfs:comment>
    </owl:Class>
    


    <!-- http://www.semanticweb.org/ontologies/2022/2/CDS_V0.6.owl#Component_Certification -->


    <owl:Class rdf:about="http://www.semanticweb.org/ontologies/2022/2/CDS_V0.6.owl#Component_Certification">
        <rdfs:subClassOf rdf:resource="http://www.semanticweb.org/ontologies/2022/2/CDS_V0.6.owl#Certification"/>
        <rdfs:comment xml:lang="en">Process and result of certifying a software component/service in order to become a certified part of the CDS infrastructure.</rdfs:comment>
    </owl:Class>
    


    <!-- http://www.semanticweb.org/ontologies/2022/2/CDS_V0.6.owl#Connector -->


    <owl:Class rdf:about="http://www.semanticweb.org/ontologies/2022/2/CDS_V0.6.owl#Connector">
        <rdfs:subClassOf rdf:resource="http://www.semanticweb.org/ontologies/2022/2/CDS_V0.6.owl#Ecosystem_Component"/>
        <rdfs:comment xml:lang="en">The Connector is communication server providing and consuming data by means of Data Apps via a number of resource Endpoints. There are different types of Connectors according to provided capabilities.</rdfs:comment>
    </owl:Class>
    


    <!-- http://www.semanticweb.org/ontologies/2022/2/CDS_V0.6.owl#Connector_Endpoint -->


    <owl:Class rdf:about="http://www.semanticweb.org/ontologies/2022/2/CDS_V0.6.owl#Connector_Endpoint">
        <rdfs:subClassOf rdf:resource="http://www.semanticweb.org/ontologies/2022/2/CDS_V0.6.owl#Endpoint"/>
        <rdfs:comment xml:lang="en">Connector-specific endpoint exposing Resources.</rdfs:comment>
    </owl:Class>
    


    <!-- http://www.semanticweb.org/ontologies/2022/2/CDS_V0.6.owl#Constraint -->


    <owl:Class rdf:about="http://www.semanticweb.org/ontologies/2022/2/CDS_V0.6.owl#Constraint">
        <rdfs:subClassOf rdf:resource="http://www.semanticweb.org/ontologies/2022/2/CDS_V0.6.owl#Abstract_Constraint"/>
        <rdfs:comment xml:lang="en">The class of Constraints that declare the conditions applicable to a rule.</rdfs:comment>
    </owl:Class>
    


    <!-- http://www.semanticweb.org/ontologies/2022/2/CDS_V0.6.owl#Contract -->


    <owl:Class rdf:about="http://www.semanticweb.org/ontologies/2022/2/CDS_V0.6.owl#Contract">
        <rdfs:comment xml:lang="en">Abstract set of rules governing the usage of a Resource.</rdfs:comment>
    </owl:Class>
    


    <!-- http://www.semanticweb.org/ontologies/2022/2/CDS_V0.6.owl#Contract_agreement -->


    <owl:Class rdf:about="http://www.semanticweb.org/ontologies/2022/2/CDS_V0.6.owl#Contract_agreement">
        <rdfs:subClassOf rdf:resource="http://www.semanticweb.org/ontologies/2022/2/CDS_V0.6.owl#Contract"/>
        <rdfs:comment xml:lang="en">Contract governing the actual usage of a Resource that has been agreed by all parties.
It represents Rules that have been granted from assigner to assignee Participant. Typically used to grant the terms of the Rules between Participants.
</rdfs:comment>
    </owl:Class>
    


    <!-- http://www.semanticweb.org/ontologies/2022/2/CDS_V0.6.owl#Contract_offer -->


    <owl:Class rdf:about="http://www.semanticweb.org/ontologies/2022/2/CDS_V0.6.owl#Contract_offer">
        <rdfs:subClassOf rdf:resource="http://www.semanticweb.org/ontologies/2022/2/CDS_V0.6.owl#Contract"/>
        <rdfs:comment xml:lang="en">Contract issued by the Data Provider offering the usage of a Resource at particular conditions.

It represents Rules that are being offered from an assigner Participant. It does not grant any Rules.</rdfs:comment>
    </owl:Class>
    


    <!-- http://www.semanticweb.org/ontologies/2022/2/CDS_V0.6.owl#Contract_request -->


    <owl:Class rdf:about="http://www.semanticweb.org/ontologies/2022/2/CDS_V0.6.owl#Contract_request">
        <rdfs:subClassOf rdf:resource="http://www.semanticweb.org/ontologies/2022/2/CDS_V0.6.owl#Contract"/>
        <rdfs:comment xml:lang="en">Contract issued by the Data Consumer requesting the usage of a Resource at particular conditions. No privileges are granted to any Party. 

It proposes a Rule over an Resource from an assignee.</rdfs:comment>
    </owl:Class>
    


    <!-- http://www.semanticweb.org/ontologies/2022/2/CDS_V0.6.owl#DataApp_Endpoint -->


    <owl:Class rdf:about="http://www.semanticweb.org/ontologies/2022/2/CDS_V0.6.owl#DataApp_Endpoint">
        <rdfs:subClassOf rdf:resource="http://www.semanticweb.org/ontologies/2022/2/CDS_V0.6.owl#Endpoint"/>
        <rdfs:comment xml:lang="en">Description of endpoints a DataApp offers.</rdfs:comment>
    </owl:Class>
    


    <!-- http://www.semanticweb.org/ontologies/2022/2/CDS_V0.6.owl#Data_App -->


    <owl:Class rdf:about="http://www.semanticweb.org/ontologies/2022/2/CDS_V0.6.owl#Data_App">
        <rdfs:subClassOf rdf:resource="http://www.semanticweb.org/ontologies/2022/2/CDS_V0.6.owl#Resource"/>
        <rdfs:comment xml:lang="en">Application - Concepts particular to Data Apps, beyond the scope of general resources, that are installed within the infrastructure in order to communicate or process data on behalf of participants of the Copernicus Data Space.</rdfs:comment>
    </owl:Class>
    


    <!-- http://www.semanticweb.org/ontologies/2022/2/CDS_V0.6.owl#Data_App_Asset -->


    <owl:Class rdf:about="http://www.semanticweb.org/ontologies/2022/2/CDS_V0.6.owl#Data_App_Asset">
        <rdfs:subClassOf rdf:resource="http://www.semanticweb.org/ontologies/2022/2/CDS_V0.6.owl#Data_App"/>
        <rdfs:comment xml:lang="en">A machine-interpretable Data Asset, such as a script file, algorithm, rule set, or another type of code, which execution relies on a particular runtime environment.</rdfs:comment>
    </owl:Class>
    


    <!-- http://www.semanticweb.org/ontologies/2022/2/CDS_V0.6.owl#Data_App_Plug-in -->


    <owl:Class rdf:about="http://www.semanticweb.org/ontologies/2022/2/CDS_V0.6.owl#Data_App_Plug-in">
        <rdfs:subClassOf rdf:resource="http://www.semanticweb.org/ontologies/2022/2/CDS_V0.6.owl#Data_App"/>
        <rdfs:comment xml:lang="en">An add-on of a Data App, adding new capabilities to it. The extension management process for selection, installation, and maintenance of such plugins has to be implemented by the respective Data App in accordance with the security policies of the Connector.</rdfs:comment>
    </owl:Class>
    


    <!-- http://www.semanticweb.org/ontologies/2022/2/CDS_V0.6.owl#Data_Asset -->


    <owl:Class rdf:about="http://www.semanticweb.org/ontologies/2022/2/CDS_V0.6.owl#Data_Asset">
        <rdfs:subClassOf rdf:resource="http://www.semanticweb.org/ontologies/2022/2/CDS_V0.6.owl#Resource"/>
        <rdfs:comment xml:lang="en">Textual documents, time series of sensor values, communication messages, archives of image files, or media streams. Data Assets are subject to forwarding, processing, or consumption.
Content exposed for exchange via Data Endpoints according to a parametrized Data Service interface; Data Assets are expected to be focused, homogeneous, and consistent over time with regard to granularity, coverage, context, data structure, and conceptual classification.</rdfs:comment>
    </owl:Class>
    


    <!-- http://www.semanticweb.org/ontologies/2022/2/CDS_V0.6.owl#Data_Service -->


    <owl:Class rdf:about="http://www.semanticweb.org/ontologies/2022/2/CDS_V0.6.owl#Data_Service">
        <rdfs:comment xml:lang="en">A Data Service is an organized system that expose Resources to Participants. It implements a set of operations that allow consumers to access data and applications, and computing and storage resources.
Data Services are all services users aim to use. The access to these services is protected and the relative usage is managed by the policy framework.</rdfs:comment>
    </owl:Class>
    


    <!-- http://www.semanticweb.org/ontologies/2022/2/CDS_V0.6.owl#Digital_Content -->


    <owl:Class rdf:about="http://www.semanticweb.org/ontologies/2022/2/CDS_V0.6.owl#Digital_Content">
        <rdfs:comment xml:lang="en">Any content of a particular type, that exists in the form of original data.</rdfs:comment>
    </owl:Class>
    


    <!-- http://www.semanticweb.org/ontologies/2022/2/CDS_V0.6.owl#Duty -->


    <owl:Class rdf:about="http://www.semanticweb.org/ontologies/2022/2/CDS_V0.6.owl#Duty">
        <rdfs:subClassOf rdf:resource="http://www.semanticweb.org/ontologies/2022/2/CDS_V0.6.owl#Rule"/>
        <rdfs:comment xml:lang="en">The obligation to exercise an Action.</rdfs:comment>
    </owl:Class>
    


    <!-- http://www.semanticweb.org/ontologies/2022/2/CDS_V0.6.owl#Ecosystem_Component -->


    <owl:Class rdf:about="http://www.semanticweb.org/ontologies/2022/2/CDS_V0.6.owl#Ecosystem_Component">
        <rdfs:subClassOf rdf:resource="http://www.semanticweb.org/ontologies/2022/2/CDS_V0.6.owl#Managed_Entity"/>
        <rdfs:comment xml:lang="en">The class of all ecosystem components of the Copernicus Data Space.</rdfs:comment>
    </owl:Class>
    


    <!-- http://www.semanticweb.org/ontologies/2022/2/CDS_V0.6.owl#Endpoint -->


    <owl:Class rdf:about="http://www.semanticweb.org/ontologies/2022/2/CDS_V0.6.owl#Endpoint">
        <rdfs:comment xml:lang="en">Access point of data exchange, service interaction and service description.</rdfs:comment>
    </owl:Class>
    


    <!-- http://www.semanticweb.org/ontologies/2022/2/CDS_V0.6.owl#Identity_Provider -->


    <owl:Class rdf:about="http://www.semanticweb.org/ontologies/2022/2/CDS_V0.6.owl#Identity_Provider">
        <rdfs:subClassOf rdf:resource="http://www.semanticweb.org/ontologies/2022/2/CDS_V0.6.owl#Ecosystem_Component"/>
        <rdfs:comment xml:lang="en">It manages and validates the digital identity of CDS Participants</rdfs:comment>
    </owl:Class>
    


    <!-- http://www.semanticweb.org/ontologies/2022/2/CDS_V0.6.owl#Logical_Constraint -->


    <owl:Class rdf:about="http://www.semanticweb.org/ontologies/2022/2/CDS_V0.6.owl#Logical_Constraint">
        <rdfs:subClassOf rdf:resource="http://www.semanticweb.org/ontologies/2022/2/CDS_V0.6.owl#Abstract_Constraint"/>
        <rdfs:comment xml:lang="en">The class of Logical Constraints that restrict a Rule. A Logical Constraints is a collection of Constraints.</rdfs:comment>
    </owl:Class>
    


    <!-- http://www.semanticweb.org/ontologies/2022/2/CDS_V0.6.owl#Managed_Entity -->


    <owl:Class rdf:about="http://www.semanticweb.org/ontologies/2022/2/CDS_V0.6.owl#Managed_Entity">
        <rdfs:comment xml:lang="en">The class of mutable individuals.</rdfs:comment>
    </owl:Class>
    


    <!-- http://www.semanticweb.org/ontologies/2022/2/CDS_V0.6.owl#Participant -->


    <owl:Class rdf:about="http://www.semanticweb.org/ontologies/2022/2/CDS_V0.6.owl#Participant">
        <rdfs:subClassOf rdf:resource="http://www.semanticweb.org/ontologies/2022/2/CDS_V0.6.owl#Managed_Entity"/>
        <rdfs:comment xml:lang="en">Process and result of certifying a software component/service in order to become a certified part of the CDS infrastructure.</rdfs:comment>
    </owl:Class>
    


    <!-- http://www.semanticweb.org/ontologies/2022/2/CDS_V0.6.owl#Participant_Certification -->


    <owl:Class rdf:about="http://www.semanticweb.org/ontologies/2022/2/CDS_V0.6.owl#Participant_Certification">
        <rdfs:subClassOf rdf:resource="http://www.semanticweb.org/ontologies/2022/2/CDS_V0.6.owl#Certification"/>
        <rdfs:comment xml:lang="en">Process and result of certifying an interested party in order to become a certified member of the CDS.</rdfs:comment>
    </owl:Class>
    


    <!-- http://www.semanticweb.org/ontologies/2022/2/CDS_V0.6.owl#Permission -->


    <owl:Class rdf:about="http://www.semanticweb.org/ontologies/2022/2/CDS_V0.6.owl#Permission">
        <rdfs:subClassOf rdf:resource="http://www.semanticweb.org/ontologies/2022/2/CDS_V0.6.owl#Rule"/>
        <rdfs:comment xml:lang="en">The ability to exercise an Action over an Resource. The Permission MAY also have the duty property that expresses an agreed Action that MUST be exercised (as a pre-condition to be granted the Permission)</rdfs:comment>
    </owl:Class>
    


    <!-- http://www.semanticweb.org/ontologies/2022/2/CDS_V0.6.owl#Person -->


    <owl:Class rdf:about="http://www.semanticweb.org/ontologies/2022/2/CDS_V0.6.owl#Person">
        <rdfs:comment xml:lang="en">The class of persons (people).</rdfs:comment>
    </owl:Class>
    


    <!-- http://www.semanticweb.org/ontologies/2022/2/CDS_V0.6.owl#Prohibition -->


    <owl:Class rdf:about="http://www.semanticweb.org/ontologies/2022/2/CDS_V0.6.owl#Prohibition">
        <rdfs:subClassOf rdf:resource="http://www.semanticweb.org/ontologies/2022/2/CDS_V0.6.owl#Rule"/>
        <rdfs:comment xml:lang="en">The inability to exercise an Action over a Resource.</rdfs:comment>
    </owl:Class>
    


    <!-- http://www.semanticweb.org/ontologies/2022/2/CDS_V0.6.owl#Resource -->


    <owl:Class rdf:about="http://www.semanticweb.org/ontologies/2022/2/CDS_V0.6.owl#Resource">
        <rdfs:subClassOf rdf:resource="http://www.semanticweb.org/ontologies/2022/2/CDS_V0.6.owl#Digital_Content"/>
        <rdfs:subClassOf rdf:resource="http://www.semanticweb.org/ontologies/2022/2/CDS_V0.6.owl#Managed_Entity"/>
        <rdfs:comment xml:lang="en">An identifiable, valuable, digital (non-physical) commodity traded and exchanged among participants by means of the infrastructure. 
Resource is a single digital content or a coherent set of digital contents. 
The Resource?s content is exposed via defined Interfaces at various protocol Endpoints.

Resources are the subject of a Rule .</rdfs:comment>
    </owl:Class>
    


    <!-- http://www.semanticweb.org/ontologies/2022/2/CDS_V0.6.owl#Rule -->


    <owl:Class rdf:about="http://www.semanticweb.org/ontologies/2022/2/CDS_V0.6.owl#Rule">
        <rdfs:comment xml:lang="en">Superclass of Permissions, Prohibitions and Duties.</rdfs:comment>
    </owl:Class>
    


    <!-- http://www.semanticweb.org/ontologies/2022/2/CDS_V0.6.owl#Service_Catalogue -->


    <owl:Class rdf:about="http://www.semanticweb.org/ontologies/2022/2/CDS_V0.6.owl#Service_Catalogue">
        <rdfs:subClassOf rdf:resource="http://www.semanticweb.org/ontologies/2022/2/CDS_V0.6.owl#Ecosystem_Component"/>
        <rdfs:comment xml:lang="en">Catalogue of all applications, services, data and software available for re-use by Third-Party users.
Note: A Web-based data catalogue is typically represented as a single instance of this class.</rdfs:comment>
    </owl:Class>
    


    <!-- http://www.semanticweb.org/ontologies/2022/2/CDS_V0.6.owl#Transaction_Data -->


    <owl:Class rdf:about="http://www.semanticweb.org/ontologies/2022/2/CDS_V0.6.owl#Transaction_Data">
        <rdfs:subClassOf rdf:resource="http://www.semanticweb.org/ontologies/2022/2/CDS_V0.6.owl#Resource"/>
        <rdfs:comment xml:lang="en">Information relevant to transaction activities.</rdfs:comment>
    </owl:Class>
    


    <!-- http://www.semanticweb.org/ontologies/2022/2/CDS_V0.6.owl#Wallet -->


    <owl:Class rdf:about="http://www.semanticweb.org/ontologies/2022/2/CDS_V0.6.owl#Wallet">
        <rdfs:subClassOf rdf:resource="http://www.semanticweb.org/ontologies/2022/2/CDS_V0.6.owl#Ecosystem_Component"/>
        <rdfs:comment xml:lang="en">Wallet Service is in charge of managing and allowing monetary / financial transaction (e.g.transfer charges)</rdfs:comment>
    </owl:Class>
    


    <!-- 
    ///////////////////////////////////////////////////////////////////////////////////////
    //
    // Individuals
    //
    ///////////////////////////////////////////////////////////////////////////////////////
     -->


    


    <!-- http://www.semanticweb.org/ontologies/2022/2/CDS_V0.6.owl#aggregate_by_consumer -->


    <owl:NamedIndividual rdf:about="http://www.semanticweb.org/ontologies/2022/2/CDS_V0.6.owl#aggregate_by_consumer">
        <rdf:type rdf:resource="http://www.semanticweb.org/ontologies/2022/2/CDS_V0.6.owl#Action"/>
    </owl:NamedIndividual>
    


    <!-- http://www.semanticweb.org/ontologies/2022/2/CDS_V0.6.owl#aggregate_by_provider -->


    <owl:NamedIndividual rdf:about="http://www.semanticweb.org/ontologies/2022/2/CDS_V0.6.owl#aggregate_by_provider">
        <rdf:type rdf:resource="http://www.semanticweb.org/ontologies/2022/2/CDS_V0.6.owl#Action"/>
    </owl:NamedIndividual>
    


    <!-- http://www.semanticweb.org/ontologies/2022/2/CDS_V0.6.owl#anonymize -->


    <owl:NamedIndividual rdf:about="http://www.semanticweb.org/ontologies/2022/2/CDS_V0.6.owl#anonymize">
        <rdf:type rdf:resource="http://www.semanticweb.org/ontologies/2022/2/CDS_V0.6.owl#Action"/>
    </owl:NamedIndividual>
    


    <!-- http://www.semanticweb.org/ontologies/2022/2/CDS_V0.6.owl#compensate -->


    <owl:NamedIndividual rdf:about="http://www.semanticweb.org/ontologies/2022/2/CDS_V0.6.owl#compensate">
        <rdf:type rdf:resource="http://www.semanticweb.org/ontologies/2022/2/CDS_V0.6.owl#Action"/>
    </owl:NamedIndividual>
    


    <!-- http://www.semanticweb.org/ontologies/2022/2/CDS_V0.6.owl#delete -->


    <owl:NamedIndividual rdf:about="http://www.semanticweb.org/ontologies/2022/2/CDS_V0.6.owl#delete">
        <rdf:type rdf:resource="http://www.semanticweb.org/ontologies/2022/2/CDS_V0.6.owl#Action"/>
    </owl:NamedIndividual>
    


    <!-- http://www.semanticweb.org/ontologies/2022/2/CDS_V0.6.owl#distribute -->


    <owl:NamedIndividual rdf:about="http://www.semanticweb.org/ontologies/2022/2/CDS_V0.6.owl#distribute">
        <rdf:type rdf:resource="http://www.semanticweb.org/ontologies/2022/2/CDS_V0.6.owl#Action"/>
    </owl:NamedIndividual>
    


    <!-- http://www.semanticweb.org/ontologies/2022/2/CDS_V0.6.owl#ecrypt -->


    <owl:NamedIndividual rdf:about="http://www.semanticweb.org/ontologies/2022/2/CDS_V0.6.owl#ecrypt">
        <rdf:type rdf:resource="http://www.semanticweb.org/ontologies/2022/2/CDS_V0.6.owl#Action"/>
    </owl:NamedIndividual>
    


    <!-- http://www.semanticweb.org/ontologies/2022/2/CDS_V0.6.owl#grant_use -->


    <owl:NamedIndividual rdf:about="http://www.semanticweb.org/ontologies/2022/2/CDS_V0.6.owl#grant_use">
        <rdf:type rdf:resource="http://www.semanticweb.org/ontologies/2022/2/CDS_V0.6.owl#Action"/>
    </owl:NamedIndividual>
    


    <!-- http://www.semanticweb.org/ontologies/2022/2/CDS_V0.6.owl#log -->


    <owl:NamedIndividual rdf:about="http://www.semanticweb.org/ontologies/2022/2/CDS_V0.6.owl#log">
        <rdf:type rdf:resource="http://www.semanticweb.org/ontologies/2022/2/CDS_V0.6.owl#Action"/>
    </owl:NamedIndividual>
    


    <!-- http://www.semanticweb.org/ontologies/2022/2/CDS_V0.6.owl#modify -->


    <owl:NamedIndividual rdf:about="http://www.semanticweb.org/ontologies/2022/2/CDS_V0.6.owl#modify">
        <rdf:type rdf:resource="http://www.semanticweb.org/ontologies/2022/2/CDS_V0.6.owl#Action"/>
    </owl:NamedIndividual>
    


    <!-- http://www.semanticweb.org/ontologies/2022/2/CDS_V0.6.owl#next_policy -->


    <owl:NamedIndividual rdf:about="http://www.semanticweb.org/ontologies/2022/2/CDS_V0.6.owl#next_policy">
        <rdf:type rdf:resource="http://www.semanticweb.org/ontologies/2022/2/CDS_V0.6.owl#Action"/>
    </owl:NamedIndividual>
    


    <!-- http://www.semanticweb.org/ontologies/2022/2/CDS_V0.6.owl#notify -->


    <owl:NamedIndividual rdf:about="http://www.semanticweb.org/ontologies/2022/2/CDS_V0.6.owl#notify">
        <rdf:type rdf:resource="http://www.semanticweb.org/ontologies/2022/2/CDS_V0.6.owl#Action"/>
    </owl:NamedIndividual>
    


    <!-- http://www.semanticweb.org/ontologies/2022/2/CDS_V0.6.owl#read -->


    <owl:NamedIndividual rdf:about="http://www.semanticweb.org/ontologies/2022/2/CDS_V0.6.owl#read">
        <rdf:type rdf:resource="http://www.semanticweb.org/ontologies/2022/2/CDS_V0.6.owl#Action"/>
    </owl:NamedIndividual>
    


    <!-- http://www.semanticweb.org/ontologies/2022/2/CDS_V0.6.owl#track_provenance -->


    <owl:NamedIndividual rdf:about="http://www.semanticweb.org/ontologies/2022/2/CDS_V0.6.owl#track_provenance">
        <rdf:type rdf:resource="http://www.semanticweb.org/ontologies/2022/2/CDS_V0.6.owl#Action"/>
    </owl:NamedIndividual>
    


    <!-- http://www.semanticweb.org/ontologies/2022/2/CDS_V0.6.owl#use -->


    <owl:NamedIndividual rdf:about="http://www.semanticweb.org/ontologies/2022/2/CDS_V0.6.owl#use">
        <rdf:type rdf:resource="http://www.semanticweb.org/ontologies/2022/2/CDS_V0.6.owl#Action"/>
    </owl:NamedIndividual>
    


    <!-- http://www.semanticweb.org/ontologies/2022/2/CDS_V0.6.owl#write -->


    <owl:NamedIndividual rdf:about="http://www.semanticweb.org/ontologies/2022/2/CDS_V0.6.owl#write">
        <rdf:type rdf:resource="http://www.semanticweb.org/ontologies/2022/2/CDS_V0.6.owl#Action"/>
    </owl:NamedIndividual>
</rdf:RDF>



<!-- Generated by the OWL API (version 5.1.14) https://github.com/owlcs/owlapi/ -->


